Authoritative DNS server derivation done.

src/Examples/DnsServer/SimplifiedAuthoritativeDNSServer.v
@@ -152,8 +152,277 @@ Qed.
 
 Local Opaque CallBagFind.
 
+    Lemma refine_Query_In_Where_False {qs_schema} {ResultT}
+      : forall Index
+               (r_o : UnConstrQueryStructure qs_schema)
+               (r_n : IndexedQueryStructure qs_schema Index)
+               idx
+               (body : _ -> Comp (list ResultT)),
+        DelegateToBag_AbsR r_o r_n
+        ->
+        refine For (UnConstrQuery_In r_o idx
+                          (fun tup : RawTuple =>
+                             Where False (body tup) ))
+               (ret [ ]).
+    Proof.
+    Admitted.
+
+
+    Lemma refine_Query_In_Where_Const {qs_schema} {ResultT} {A}
+          {_ : @Query_eq A}
+      : forall Index
+               (r_o : UnConstrQueryStructure qs_schema)
+               (r_n : IndexedQueryStructure qs_schema Index)
+               idx
+               (body : _ -> Comp (list ResultT))
+               Q a a',
+        DelegateToBag_AbsR r_o r_n
+        -> refine For (UnConstrQuery_In r_o idx
+                                     (fun tup : RawTuple =>
+                                        Where (a = a' /\ Q tup)
+                                              (body tup) ))
+               (If A_eq_dec a a' Then
+                   For (UnConstrQuery_In r_o idx
+                                     (fun tup : RawTuple =>
+                                        Where (Q tup)
+                                              (body tup) ))
+                   Else
+                   (ret [ ])).
+    Proof.
+    Admitted.
+
+    Corollary refine_Count_Query_In_Where_False {qs_schema} {ResultT}
+      : forall Index
+               (r_o : UnConstrQueryStructure qs_schema)
+               (r_n : IndexedQueryStructure qs_schema Index)
+               idx
+               (body : _ -> Comp (list ResultT)),
+        DelegateToBag_AbsR r_o r_n
+        ->
+        refine (Count For (UnConstrQuery_In r_o idx
+                          (fun tup : RawTuple =>
+                             Where False (body tup) )))
+               (ret 0).
+    Proof.
+      intros; rewrite refine_Query_In_Where_False; simpl; eauto.
+      rewrite refine_Count; simplify with monad laws; reflexivity.
+    Qed.
+
+    Corollary refine_Count_Query_In_Where_Const {qs_schema} {ResultT} {A}
+          {_ : @Query_eq A}
+      : forall Index
+               (r_o : UnConstrQueryStructure qs_schema)
+               (r_n : IndexedQueryStructure qs_schema Index)
+               idx
+               (body : _ -> Comp (list ResultT))
+               Q a a',
+        DelegateToBag_AbsR r_o r_n
+        -> refine (Count For (UnConstrQuery_In r_o idx
+                                     (fun tup : RawTuple =>
+                                        Where (a = a' /\ Q tup)
+                                              (body tup) )))
+               (If A_eq_dec a a' Then
+                   (Count For (UnConstrQuery_In r_o idx
+                                     (fun tup : RawTuple =>
+                                        Where (Q tup)
+                                              (body tup) )))
+                   Else
+                   (ret 0)).
+    Proof.
+      intros; rewrite refine_Query_In_Where_Const; eauto.
+      find_if_inside; simpl; eauto.
+      reflexivity.
+      rewrite refine_Count; simplify with monad laws; reflexivity.
+    Qed.
+
+    Lemma refine_Query_In_Where_Const_neq {qs_schema} {ResultT} {A}
+          {_ : @Query_eq A}
+      : forall Index
+               (r_o : UnConstrQueryStructure qs_schema)
+               (r_n : IndexedQueryStructure qs_schema Index)
+               idx
+               (body : _ -> Comp (list ResultT))
+               Q a a',
+        DelegateToBag_AbsR r_o r_n
+        -> refine For (UnConstrQuery_In r_o idx
+                                     (fun tup : RawTuple =>
+                                        Where (a <> a' /\ Q tup)
+                                              (body tup) ))
+               (If A_eq_dec a a' Then
+                   (ret [ ])
+                   Else
+                   For (UnConstrQuery_In r_o idx
+                                         (fun tup : RawTuple =>
+                                            Where (Q tup)
+                                                  (body tup) ))
+).
+    Proof.
+    Admitted.
+
+    Corollary refine_Count_Query_In_Where_Const_neq {qs_schema} {ResultT} {A}
+          {_ : @Query_eq A}
+      : forall Index
+               (r_o : UnConstrQueryStructure qs_schema)
+               (r_n : IndexedQueryStructure qs_schema Index)
+               idx
+               (body : _ -> Comp (list ResultT))
+               Q a a',
+        DelegateToBag_AbsR r_o r_n
+        -> refine (Count For (UnConstrQuery_In r_o idx
+                                     (fun tup : RawTuple =>
+                                        Where (a <> a' /\ Q tup)
+                                              (body tup) )))
+               (If A_eq_dec a a' Then
+                   (ret 0)
+                   Else
+                   (Count For (UnConstrQuery_In r_o idx
+                                                (fun tup : RawTuple =>
+                                                   Where (Q tup)
+                                                         (body tup) )))).
+    Proof.
+      intros; rewrite refine_Query_In_Where_Const_neq; eauto.
+      find_if_inside; simpl; eauto.
+      rewrite refine_Count; simplify with monad laws; reflexivity.
+      reflexivity.
+    Qed.
+
+Lemma refine_MaxPrefix {resultT}
+  : forall (f : resultT -> string) (l : Comp (list resultT)),
+    refine (MaxElements (fun s s' => prefix (f s) (f s')) l)
+           (results <- l;
+              ret (snd (@fold_left (prod string (list resultT)) resultT
+                                   (fun maxes s => If prefix (fst maxes) (f s) Then
+                                                      (If prefix (f s) (fst maxes) Then (fst maxes, s :: (snd maxes))
+                                                          Else (f s, [s]))
+                                                      Else maxes) results ("", [ ])))).
+Proof.
+Admitted.
+
+    Ltac implement_Count find_search_term ::=
+  match goal with
+    [ H : @DelegateToBag_AbsR ?qs_schema ?indices ?r_o ?r_n
+      |- refine (Bind (Count For (UnConstrQuery_In _ ?idx (fun tup => Where (@?P tup) Return (@?f tup))))
+                 _) _ ] =>
+    let filter_dec := eval simpl in (@DecideableEnsembles.dec _ P _) in
+        let idx_search_update_term := eval simpl in (ith3 indices idx) in
+            let search_term_type' := eval simpl in (BagSearchTermType idx_search_update_term) in
+                let search_term_matcher := eval simpl in (BagMatchSearchTerm idx_search_update_term) in
+                    makeEvar search_term_type'
+                             ltac: (fun search_term =>
+                                      let eqv := fresh in
+                                      assert (ExtensionalEq filter_dec (search_term_matcher search_term)) as eqv;
+                                      [ find_search_term qs_schema idx filter_dec search_term
+                                      |
+                                      let H' := fresh in
+                                      pose proof (@refine_BagFindBagCount
+                                                    _
+                                                   qs_schema indices
+                                                   idx r_o r_n search_term P f H eqv) as H';
+                                      fold_string_hyps_in H'; fold_heading_hyps_in H';
+                                      rewrite H'; clear H' eqv
+                                   ])
+  | [ H : @DelegateToBag_AbsR ?qs_schema ?indices ?r_o ?r_n
+      |- refine (Bind (Count For (UnConstrQuery_In _ ?idx (fun tup => Where (@?P tup) Return _)))
+                 _) _ ] =>
+    let filter_dec := eval simpl in (@DecideableEnsembles.dec _ P _) in
+        let idx_search_update_term := eval simpl in (ith3 indices idx) in
+            let search_term_type' := eval simpl in (BagSearchTermType idx_search_update_term) in
+                let search_term_matcher := eval simpl in (BagMatchSearchTerm idx_search_update_term) in
+                    makeEvar search_term_type'
+                             ltac: (fun search_term =>
+                                      let eqv := fresh in
+                                      assert (ExtensionalEq filter_dec (search_term_matcher search_term)) as eqv;
+                                      [ find_search_term qs_schema idx filter_dec search_term
+                                      |
+                                      let H' := fresh in
+                                      pose proof (@refine_BagFindBagCount unit
+                                                   qs_schema indices
+                                                   idx r_o r_n search_term P (fun _ => tt) _ H eqv) as H';
+                                      fold_string_hyps_in H'; fold_heading_hyps_in H';
+                                      rewrite H'; clear H' eqv
+                                      ])
+  end.
+
+
+Ltac implement_insert''' :=
+  first [ implement_simple_For
+            ltac:(find_simple_search_term
+            ltac:(CombineCase5 StringPrefixIndexUse EqIndexUse)
+            ltac:(CombineCase10 createEarlyStringPrefixTerm createEarlyEqualityTerm)
+            ltac:(CombineCase7 createLastStringPrefixTerm createLastEqualityTerm))
+        | implement_Count
+            ltac:(find_simple_search_term
+            ltac:(CombineCase5 StringPrefixIndexUse EqIndexUse)
+            ltac:(CombineCase10 createEarlyStringPrefixTerm createEarlyEqualityTerm)
+            ltac:(CombineCase7 createLastStringPrefixTerm createLastEqualityTerm))
+        | implement_insert''].
+
+
+Ltac  simplify_Query_Where ::=
+    match goal with
+    |- context [UnConstrQuery_In ?r_n ?Ridx (fun tup =>  Query_Where (@?P tup) _)] =>
+    rewrite (fun ResultT =>
+               @refine_UnConstrQuery_In_Query_Where_Cond _ r_n Ridx ResultT P);
+      [ | intros;
+          match goal with
+            |- context [RDataTypeToRRecordType (SumType.inj_SumType ?y ?z ?x) <> ?q] =>
+            case_eq (fin_eq_dec z q); simpl; intros ? ?; try discriminate;
+            first [let H' := fresh in
+                   assert (RDataTypeToRRecordType (SumType.inj_SumType y z x) <> q <-> True) as H' by
+                         (rewrite RDataTypeToRRecordType_inj; intuition eauto);
+                   set_evars; rewrite ?H', ?and_True_l, ?and_True_r, ?and_False_r, ?and_False_l
+                  | let H' := fresh in
+                    assert (RDataTypeToRRecordType (SumType.inj_SumType y z x) <> q <-> False) as H' by
+                          (rewrite RDataTypeToRRecordType_inj; eauto; intuition eauto);
+                    set_evars; rewrite ?H', ?and_True_l, ?and_True_r, ?and_False_r, ?and_False_l];
+            finish honing
+          | |- context [RDataTypeToRRecordType (SumType.inj_SumType ?y ?z ?x) = ?q] =>
+            case_eq (fin_eq_dec z q); simpl; intros ? ?; try discriminate;
+            first [let H' := fresh in
+                   assert (RDataTypeToRRecordType (SumType.inj_SumType y z x) = q <-> True) as H' by
+                         (rewrite RDataTypeToRRecordType_inj; intuition eauto);
+                   set_evars; rewrite ?H', ?and_True_l, ?and_True_r, ?and_False_r, ?and_False_l
+                  | let H' := fresh in
+                    assert (RDataTypeToRRecordType (SumType.inj_SumType y z x) = q <-> False) as H' by
+                          (rewrite RDataTypeToRRecordType_inj; eauto; intuition eauto);
+                    set_evars; rewrite ?H', ?and_True_l, ?and_True_r, ?and_False_r, ?and_False_l
+                  | rewrite RDataTypeToRRecordType_inj; eauto];
+            finish honing
+          | |- context [RDataTypeToRRecordType (SumType.inj_SumType ?y ?z ?x)] =>
+            set_evars; rewrite !RDataTypeToRRecordType_inj; eauto; finish honing
+          end]
+    end.
+
+    Ltac simplify_Query_Where' :=
+      match goal with
+      H : DelegateToBag_AbsR ?r_o ?r_n
+      |- refine (Bind (For (UnConstrQuery_In ?r_o ?idx
+                                             (fun tup => Where False (@?body tup)))) _)
+                _ => rewrite (@refine_Query_In_Where_False _ _ _ r_o r_n idx body H)
+      | H : DelegateToBag_AbsR ?r_o ?r_n
+      |- refine (Bind (For (UnConstrQuery_In (qsSchema := ?qs_schema) ?r_o ?idx
+                                             (fun tup => Where (?a = ?b /\ @?Q tup) (@?body tup)))) _)
+                _ => rewrite (@refine_Query_In_Where_Const qs_schema _ _ _ _ r_o _ idx body Q a b H)
+      | H : DelegateToBag_AbsR ?r_o ?r_n
+        |- refine (Bind (For (UnConstrQuery_In (qsSchema := ?qs_schema) ?r_o ?idx
+                                             (fun tup => Where (?a <> ?b /\ @?Q tup) (@?body tup)))) _)
+                _ => rewrite (@refine_Query_In_Where_Const_neq qs_schema _ _ _ _ r_o _ idx body Q a b H)
+      | H : DelegateToBag_AbsR ?r_o ?r_n
+      |- refine (Bind (Count (For (UnConstrQuery_In ?r_o ?idx
+                                             (fun tup => Where False (@?body tup))))) _)
+                _ => rewrite (@refine_Count_Query_In_Where_False _ _ _ r_o r_n idx body H)
+      | H : DelegateToBag_AbsR ?r_o ?r_n
+      |- refine (Bind (Count (For (UnConstrQuery_In (qsSchema := ?qs_schema) ?r_o ?idx
+                                             (fun tup => Where (?a = ?b /\ @?Q tup) (@?body tup))))) _)
+                _ => rewrite (@refine_Count_Query_In_Where_Const qs_schema _ _ _ _ r_o _ idx body Q a b H)
+      | H : DelegateToBag_AbsR ?r_o ?r_n
+      |- refine (Bind (Count (For (UnConstrQuery_In (qsSchema := ?qs_schema) ?r_o ?idx
+                                             (fun tup => Where (?a <> ?b /\ @?Q tup) (@?body tup))))) _)
+                _ => rewrite (@refine_Count_Query_In_Where_Const_neq qs_schema _ _ _ _ r_o _ idx body Q a b H)
+    end.
+
 Theorem DnsManual :
-  FullySharpened DnsSpec.
+  {DnsImpl : _ & refineADT DnsSpec DnsImpl}.
 Proof.
   eexists; unfold DnsSpec.
   pose_string_hyps; pose_heading_hyps.
@@ -493,13 +762,14 @@ Proof.
     doOne ltac:(drop_constraints)
                  drop_constraints_drill ltac:(repeat subst_refine_evar; cbv beta; simpl; try finish honing).
     simpl.
+    Local Transparent UpdateUnConstrRelationInsertC.
+
     erewrite (DecomposeRawQueryStructureSchema_UpdateUnConstrRelationInsertC_eq _ _ H0);
       [ | eassumption | intros; set_refine_evar; refine pick val (snd r_n'); destruct r_n';
                         try eauto;
                         simplify with monad laws; simpl; try finish honing;
                         unfold H8; instantiate (1 := fun z => ret (snd z, true)); reflexivity].
     simpl.
-    Local Transparent UpdateUnConstrRelationInsertC.
     unfold UpdateUnConstrRelationInsertC at 1.
     doOne ltac:(drop_constraints)
                  drop_constraints_drill ltac:(repeat subst_refine_evar; cbv beta; simpl; try finish honing).
@@ -698,7 +968,9 @@ Proof.
                         drop_constraints_drill ltac:(repeat subst_refine_evar; cbv beta; simpl; try finish honing).
     refine pick val _; eauto; finish honing.
   }
-  { destruct_ex.
+  { (* Process *)
+
+    destruct_ex.
     doOne ltac:(drop_constraints)
                  drop_constraints_drill ltac:(repeat subst_refine_evar; cbv beta; simpl; try finish honing).
     doOne ltac:(drop_constraints)
@@ -718,7 +990,6 @@ Proof.
     doOne ltac:(drop_constraints)
                  drop_constraints_drill ltac:(repeat subst_refine_evar; cbv beta; simpl; try finish honing).
     rewrite (refine_QueryIn_Where _ _ H0).
-
     simplify_GetAttributeRaw_inj.
     rewrite (UnConstrQuery_In_Where_Map).
     rewrite refine_For_Map.
@@ -765,14 +1036,7 @@ Proof.
     repeat doOne ltac:(drop_constraints)
                  drop_constraints_drill ltac:(repeat subst_refine_evar; cbv beta; simpl; try finish honing).
     refine pick val _; eauto.
-    doOne ltac:(drop_constraints)
-                 drop_constraints_drill ltac:(repeat subst_refine_evar; cbv beta; simpl; try finish honing).
-
-    doOne ltac:(drop_constraints)
-                 drop_constraints_drill ltac:(repeat subst_refine_evar; cbv beta; simpl; try finish honing).
-    doOne ltac:(drop_constraints)
-                 drop_constraints_drill ltac:(repeat subst_refine_evar; cbv beta; simpl; try finish honing).
-    doOne ltac:(drop_constraints)
+    repeat doOne ltac:(drop_constraints)
                  drop_constraints_drill ltac:(repeat subst_refine_evar; cbv beta; simpl; try finish honing).
     setoid_rewrite refine_If_Then_Bind.
     rewrite refine_Process_Query_Exact_Match by eassumption.
@@ -875,13 +1139,12 @@ Proof.
     simplify_GetAttributeRaw_inj.
     repeat doOne ltac:(drop_constraints)
                  drop_constraints_drill ltac:(repeat subst_refine_evar; cbv beta; simpl; try finish honing).
-    doOne ltac:(drop_constraints)
+    repeat doOne ltac:(drop_constraints)
                  drop_constraints_drill ltac:(repeat subst_refine_evar; cbv beta; simpl; try finish honing).
     doOne ltac:(drop_constraints)
                  drop_constraints_drill ltac:(repeat subst_refine_evar; cbv beta; simpl; try finish honing).
     doOne ltac:(drop_constraints)
                  drop_constraints_drill ltac:(repeat subst_refine_evar; cbv beta; simpl; try finish honing).
-    
     doOne ltac:(drop_constraints)
                  drop_constraints_drill ltac:(repeat subst_refine_evar; cbv beta; simpl; try finish honing).
     doOne ltac:(drop_constraints)
@@ -892,89 +1155,67 @@ Proof.
                  drop_constraints_drill ltac:(repeat subst_refine_evar; cbv beta; simpl; try finish honing).
     doOne ltac:(drop_constraints)
                  drop_constraints_drill ltac:(repeat subst_refine_evar; cbv beta; simpl; try finish honing).
-    simplify_GetAttributeRaw_inj.
-    simplify_GetAttributeRaw_inj.
-    simpl; simplify_Query_Where.
 
+    repeat first
+           [ simplify_GetAttributeRaw_inj
+           | simplify_Query_Where ].
     doOne ltac:(drop_constraints)
                  drop_constraints_drill ltac:(repeat subst_refine_evar; cbv beta; simpl; try finish honing).
     doOne ltac:(drop_constraints)
                  drop_constraints_drill ltac:(repeat subst_refine_evar; cbv beta; simpl; try finish honing).
-    simplify_GetAttributeRaw_inj.
-    simplify_GetAttributeRaw_inj.
-    simpl; simplify_Query_Where.
+    repeat first
+           [ simplify_GetAttributeRaw_inj
+           | simplify_Query_Where ].
     doOne ltac:(drop_constraints)
                  drop_constraints_drill ltac:(repeat subst_refine_evar; cbv beta; simpl; try finish honing).
     doOne ltac:(drop_constraints)
                  drop_constraints_drill ltac:(repeat subst_refine_evar; cbv beta; simpl; try finish honing).
-    simplify_GetAttributeRaw_inj.
-    simplify_GetAttributeRaw_inj.
-    simplify_Query_Where.
+    repeat first
+           [ simplify_GetAttributeRaw_inj
+           | simplify_Query_Where ].
     doOne ltac:(drop_constraints)
                  drop_constraints_drill ltac:(repeat subst_refine_evar; cbv beta; simpl; try finish honing).
     doOne ltac:(drop_constraints)
                  drop_constraints_drill ltac:(repeat subst_refine_evar; cbv beta; simpl; try finish honing).
-    simplify_GetAttributeRaw_inj.
-    simplify_GetAttributeRaw_inj.
-    simplify_Query_Where.
-    doOne ltac:(drop_constraints)
+    repeat first
+           [ simplify_GetAttributeRaw_inj
+           | simplify_Query_Where ].
+    repeat doOne ltac:(drop_constraints)
                  drop_constraints_drill ltac:(repeat subst_refine_evar; cbv beta; simpl; try finish honing).
-    doOne ltac:(drop_constraints)
+    repeat doOne ltac:(drop_constraints)
                  drop_constraints_drill ltac:(repeat subst_refine_evar; cbv beta; simpl; try finish honing).
-    doOne ltac:(drop_constraints)
-                 drop_constraints_drill ltac:(repeat subst_refine_evar; cbv beta; simpl; try finish honing).
-    rewrite (refine_Iterate_Count_For_UnConstrQuery_In _ H0).
-    unfold Iterate_Equiv_Count_For_UnConstrQuery_In_body; simpl.
-    doOne ltac:(drop_constraints)
-                 drop_constraints_drill ltac:(repeat subst_refine_evar; cbv beta; simpl; try finish honing).
-    doOne ltac:(drop_constraints)
-                 drop_constraints_drill ltac:(repeat subst_refine_evar; cbv beta; simpl; try finish honing).
-    simplify_GetAttributeRaw_inj.
-    simplify_GetAttributeRaw_inj.
-    simpl; simplify_Query_Where.
-    simpl; simplify_Query_Where.
+    - rewrite (refine_Iterate_Count_For_UnConstrQuery_In _ H0).
+      unfold Iterate_Equiv_Count_For_UnConstrQuery_In_body; simpl.
+      doOne ltac:(drop_constraints)
+                   drop_constraints_drill ltac:(repeat subst_refine_evar; cbv beta; simpl; try finish honing).
+      doOne ltac:(drop_constraints)
+                   drop_constraints_drill ltac:(repeat subst_refine_evar; cbv beta; simpl; try finish honing).
+      repeat first
+             [ simplify_GetAttributeRaw_inj
+             | simplify_Query_Where ].
     repeat doOne ltac:(drop_constraints)
                  drop_constraints_drill ltac:(repeat subst_refine_evar; cbv beta; simpl; try finish honing).
     doOne ltac:(drop_constraints)
                  drop_constraints_drill ltac:(repeat subst_refine_evar; cbv beta; simpl; try finish honing).
-    simplify_GetAttributeRaw_inj.
-    simplify_GetAttributeRaw_inj.
-    simpl; simplify_Query_Where.
-
-  match goal with
-    |- context [UnConstrQuery_In ?r_n ?Ridx (fun tup =>  Query_Where (@?P tup) _)] =>
-    rewrite (fun ResultT =>
-               @refine_UnConstrQuery_In_Query_Where_Cond _ r_n Ridx ResultT P);
-      [ | intros; rewrite RDataTypeToRRecordType_inj; finish honing]
-  end.
-  doOne ltac:(drop_constraints)
+    repeat first
+           [ simplify_GetAttributeRaw_inj
+           | simplify_Query_Where ].
+    repeat doOne ltac:(drop_constraints)
                  drop_constraints_drill ltac:(repeat subst_refine_evar; cbv beta; simpl; try finish honing).
-
       doOne ltac:(drop_constraints)
                  drop_constraints_drill ltac:(repeat subst_refine_evar; cbv beta; simpl; try finish honing).
-    simplify_GetAttributeRaw_inj.
-    simplify_GetAttributeRaw_inj.
-    simpl; simplify_Query_Where.
-    match goal with
-    |- context [UnConstrQuery_In ?r_n ?Ridx (fun tup =>  Query_Where (@?P tup) _)] =>
-    rewrite (fun ResultT =>
-               @refine_UnConstrQuery_In_Query_Where_Cond _ r_n Ridx ResultT P);
-      [ | intros; rewrite RDataTypeToRRecordType_inj; finish honing]
-  end.
-    finish honing.
+    repeat first
+           [ simplify_GetAttributeRaw_inj
+           | simplify_Query_Where ].
+    repeat doOne ltac:(drop_constraints)
+                 drop_constraints_drill ltac:(repeat subst_refine_evar; cbv beta; simpl; try finish honing).
     doOne ltac:(drop_constraints)
                  drop_constraints_drill ltac:(repeat subst_refine_evar; cbv beta; simpl; try finish honing).
-    simplify_GetAttributeRaw_inj.
-    simplify_GetAttributeRaw_inj.
-    simpl; simplify_Query_Where.
-    match goal with
-    |- context [UnConstrQuery_In ?r_n ?Ridx (fun tup =>  Query_Where (@?P tup) _)] =>
-    rewrite (fun ResultT =>
-               @refine_UnConstrQuery_In_Query_Where_Cond _ r_n Ridx ResultT P);
-      [ | intros; rewrite RDataTypeToRRecordType_inj; finish honing]
-  end.
-    finish honing.
-    finish honing.
+    repeat first
+           [ simplify_GetAttributeRaw_inj
+           | simplify_Query_Where ].
+    repeat doOne ltac:(drop_constraints)
+                        drop_constraints_drill ltac:(repeat subst_refine_evar; cbv beta; simpl; try finish honing).
     doOne ltac:(drop_constraints)
                  drop_constraints_drill ltac:(repeat subst_refine_evar; cbv beta; simpl; try finish honing).
     doOne ltac:(drop_constraints)
@@ -1033,6 +1274,7 @@ Proof.
                  drop_constraints_drill ltac:(repeat subst_refine_evar; cbv beta; simpl; try finish honing).
     doOne ltac:(drop_constraints)
                  drop_constraints_drill ltac:(repeat subst_refine_evar; cbv beta; simpl; try finish honing).
+    - simpl.
     etransitivity.
     doOne ltac:(drop_constraints)
                  drop_constraints_drill ltac:(repeat subst_refine_evar; cbv beta; simpl; try finish honing).
@@ -1087,15 +1329,15 @@ Proof.
                  drop_constraints_drill ltac:(repeat subst_refine_evar; cbv beta; simpl; try finish honing).
     doOne ltac:(drop_constraints)
                  drop_constraints_drill ltac:(repeat subst_refine_evar; cbv beta; simpl; try finish honing).
-    simpl.
+    - simpl.
     finish honing.
 
-    repeat doOne ltac:(drop_constraints)
+    - repeat doOne ltac:(drop_constraints)
                  drop_constraints_drill ltac:(repeat subst_refine_evar; cbv beta; simpl; try finish honing).
-    refine pick val _; eauto; finish honing.
-    repeat doOne ltac:(drop_constraints)
-                 drop_constraints_drill ltac:(repeat subst_refine_evar; cbv beta; simpl; try finish honing).
-    refine pick val _; eauto; finish honing.
+      refine pick val _; eauto; finish honing.
+    - repeat doOne ltac:(drop_constraints)
+                          drop_constraints_drill ltac:(repeat subst_refine_evar; cbv beta; simpl; try finish honing).
+      refine pick val _; eauto; finish honing.
   }
   simpl.
   pose {| prim_fst := [(EqualityIndex, @Fin.F1 3);
@@ -1170,2072 +1412,679 @@ Proof.
     eauto.
   }
   { (* Process *)
-    doOne ltac:(first [
-                implement_Count
-                  ltac:(find_simple_search_term
-                          ltac:(CombineCase5 StringPrefixIndexUse EqIndexUse)
-                                 ltac:(CombineCase10 createEarlyStringPrefixTerm createEarlyEqualityTerm)
-                                        ltac:(CombineCase7 createLastStringPrefixTerm createLastEqualityTerm))
-              | implement_insert''])
+
+    doOne implement_insert'''
           ltac:(master_implement_drill
           ltac:(CombineCase5 StringPrefixIndexUse EqIndexUse)
           ltac:(CombineCase10 createEarlyStringPrefixTerm createEarlyEqualityTerm)
           ltac:(CombineCase7 createLastStringPrefixTerm createLastEqualityTerm);
                 set_evars) ltac:(finish honing).
-    doOne ltac:(first [
-                implement_Count
-                  ltac:(find_simple_search_term
-                          ltac:(CombineCase5 StringPrefixIndexUse EqIndexUse)
-                                 ltac:(CombineCase10 createEarlyStringPrefixTerm createEarlyEqualityTerm)
-                                        ltac:(CombineCase7 createLastStringPrefixTerm createLastEqualityTerm))
-              | implement_insert''])
+    doOne implement_insert'''
           ltac:(master_implement_drill
           ltac:(CombineCase5 StringPrefixIndexUse EqIndexUse)
           ltac:(CombineCase10 createEarlyStringPrefixTerm createEarlyEqualityTerm)
           ltac:(CombineCase7 createLastStringPrefixTerm createLastEqualityTerm);
                 set_evars) ltac:(finish honing).
-    repeat doOne ltac:(first [
-                implement_Count
-                  ltac:(find_simple_search_term
-                          ltac:(CombineCase5 StringPrefixIndexUse EqIndexUse)
-                                 ltac:(CombineCase10 createEarlyStringPrefixTerm createEarlyEqualityTerm)
-                                        ltac:(CombineCase7 createLastStringPrefixTerm createLastEqualityTerm))
-              | implement_insert''])
+    doOne implement_insert'''
+          ltac:(master_implement_drill
+          ltac:(CombineCase5 StringPrefixIndexUse EqIndexUse)
+          ltac:(CombineCase10 createEarlyStringPrefixTerm createEarlyEqualityTerm)
+          ltac:(CombineCase7 createLastStringPrefixTerm createLastEqualityTerm);
+                set_evars) ltac:(finish honing).
+    doOne implement_insert'''
+          ltac:(master_implement_drill
+          ltac:(CombineCase5 StringPrefixIndexUse EqIndexUse)
+          ltac:(CombineCase10 createEarlyStringPrefixTerm createEarlyEqualityTerm)
+          ltac:(CombineCase7 createLastStringPrefixTerm createLastEqualityTerm);
+                set_evars) ltac:(finish honing).
+    doOne implement_insert'''
+          ltac:(master_implement_drill
+          ltac:(CombineCase5 StringPrefixIndexUse EqIndexUse)
+          ltac:(CombineCase10 createEarlyStringPrefixTerm createEarlyEqualityTerm)
+          ltac:(CombineCase7 createLastStringPrefixTerm createLastEqualityTerm);
+                set_evars) ltac:(finish honing).
+    doOne implement_insert'''
+          ltac:(master_implement_drill
+          ltac:(CombineCase5 StringPrefixIndexUse EqIndexUse)
+          ltac:(CombineCase10 createEarlyStringPrefixTerm createEarlyEqualityTerm)
+          ltac:(CombineCase7 createLastStringPrefixTerm createLastEqualityTerm);
+                set_evars) ltac:(finish honing).
+    doOne implement_insert'''
           ltac:(master_implement_drill
           ltac:(CombineCase5 StringPrefixIndexUse EqIndexUse)
           ltac:(CombineCase10 createEarlyStringPrefixTerm createEarlyEqualityTerm)
           ltac:(CombineCase7 createLastStringPrefixTerm createLastEqualityTerm);
                 set_evars) ltac:(finish honing).
     drop_constraints.
-    repeat doOne ltac:(first [
-                implement_Count
-                  ltac:(find_simple_search_term
-                          ltac:(CombineCase5 StringPrefixIndexUse EqIndexUse)
-                                 ltac:(CombineCase10 createEarlyStringPrefixTerm createEarlyEqualityTerm)
-                                        ltac:(CombineCase7 createLastStringPrefixTerm createLastEqualityTerm))
-              | implement_insert''])
+    doOne implement_insert'''
           ltac:(master_implement_drill
           ltac:(CombineCase5 StringPrefixIndexUse EqIndexUse)
           ltac:(CombineCase10 createEarlyStringPrefixTerm createEarlyEqualityTerm)
           ltac:(CombineCase7 createLastStringPrefixTerm createLastEqualityTerm);
                 set_evars) ltac:(finish honing).
-    doOne ltac:(first [
-                implement_Count
-                  ltac:(find_simple_search_term
-                          ltac:(CombineCase5 StringPrefixIndexUse EqIndexUse)
-                                 ltac:(CombineCase10 createEarlyStringPrefixTerm createEarlyEqualityTerm)
-                                        ltac:(CombineCase7 createLastStringPrefixTerm createLastEqualityTerm))
-              | implement_insert''])
+    doOne implement_insert'''
           ltac:(master_implement_drill
           ltac:(CombineCase5 StringPrefixIndexUse EqIndexUse)
           ltac:(CombineCase10 createEarlyStringPrefixTerm createEarlyEqualityTerm)
           ltac:(CombineCase7 createLastStringPrefixTerm createLastEqualityTerm);
                 set_evars) ltac:(finish honing).
-    repeat doOne ltac:(first [
-                    implement_Count
-                      ltac:(find_simple_search_term
-                              ltac:(CombineCase5 StringPrefixIndexUse EqIndexUse)
-                                     ltac:(CombineCase10 createEarlyStringPrefixTerm createEarlyEqualityTerm)
-                                            ltac:(CombineCase7 createLastStringPrefixTerm createLastEqualityTerm))
-                  | implement_insert''])
-                 ltac:(master_implement_drill
-                         ltac:(CombineCase5 StringPrefixIndexUse EqIndexUse)
-                                ltac:(CombineCase10 createEarlyStringPrefixTerm createEarlyEqualityTerm)
-                                       ltac:(CombineCase7 createLastStringPrefixTerm createLastEqualityTerm);
-                       set_evars) ltac:(finish honing).
-    doOne ltac:(first [
-                    implement_Count
-                      ltac:(find_simple_search_term
-                              ltac:(CombineCase5 StringPrefixIndexUse EqIndexUse)
-                                     ltac:(CombineCase10 createEarlyStringPrefixTerm createEarlyEqualityTerm)
-                                            ltac:(CombineCase7 createLastStringPrefixTerm createLastEqualityTerm))
-                  | implement_insert''])
-                 ltac:(master_implement_drill
-                         ltac:(CombineCase5 StringPrefixIndexUse EqIndexUse)
-                                ltac:(CombineCase10 createEarlyStringPrefixTerm createEarlyEqualityTerm)
-                                       ltac:(CombineCase7 createLastStringPrefixTerm createLastEqualityTerm);
-                       set_evars) ltac:(finish honing).
-    doOne ltac:(first [
-                    implement_Count
-                      ltac:(find_simple_search_term
-                              ltac:(CombineCase5 StringPrefixIndexUse EqIndexUse)
-                                     ltac:(CombineCase10 createEarlyStringPrefixTerm createEarlyEqualityTerm)
-                                            ltac:(CombineCase7 createLastStringPrefixTerm createLastEqualityTerm))
-                  | implement_insert''])
-                 ltac:(master_implement_drill
-                         ltac:(CombineCase5 StringPrefixIndexUse EqIndexUse)
-                                ltac:(CombineCase10 createEarlyStringPrefixTerm createEarlyEqualityTerm)
-                                       ltac:(CombineCase7 createLastStringPrefixTerm createLastEqualityTerm);
-                       set_evars) ltac:(finish honing).
-    
-    
-    destruct_ex.
-    doOne ltac:(drop_constraints)
-                 drop_constraints_drill ltac:(repeat subst_refine_evar; cbv beta; simpl; try finish honing).
-    doOne ltac:(drop_constraints)
-                 drop_constraints_drill ltac:(repeat subst_refine_evar; cbv beta; simpl; try finish honing).
-    doOne ltac:(drop_constraints)
-                 drop_constraints_drill ltac:(repeat subst_refine_evar; cbv beta; simpl; try finish honing).
-    doOne ltac:(drop_constraints)
-                 drop_constraints_drill ltac:(repeat subst_refine_evar; cbv beta; simpl; try finish honing).
-    doOne ltac:(drop_constraints)
-                 drop_constraints_drill ltac:(repeat subst_refine_evar; cbv beta; simpl; try finish honing).
-    doOne ltac:(drop_constraints)
-                 drop_constraints_drill ltac:(repeat subst_refine_evar; cbv beta; simpl; try finish honing).
-    doOne ltac:(drop_constraints)
-                 drop_constraints_drill ltac:(repeat subst_refine_evar; cbv beta; simpl; try finish honing).
-    doOne ltac:(drop_constraints)
-                 drop_constraints_drill ltac:(repeat subst_refine_evar; cbv beta; simpl; try finish honing).
-    doOne ltac:(drop_constraints)
-                 drop_constraints_drill ltac:(repeat subst_refine_evar; cbv beta; simpl; try finish honing).
-    rewrite (refine_QueryIn_Where _ _ H0).
-    rewrite (UnConstrQuery_In_Where_Map).
-    rewrite refine_For_Map.
-    doOne ltac:(drop_constraints)
-                 drop_constraints_drill ltac:(repeat subst_refine_evar; cbv beta; simpl; try finish honing).
-    drop_constraints_drill.
-    simpl; finish honing.
-    etransitivity.
-    eapply refine_If_opt_hd_error_map; intros; try eauto.
-    match goal with
-      |- refine (If_Then_Else ?c _ _) _ =>
-      subst_refine_evar; eapply refine_if with (b := c);
-        let H := fresh in
-        intro H; set_refine_evar; try rewrite H; simpl
-    end.
-    rewrite refine_decides_QType_match by eauto.
-    simplify with monad laws.
-    find_if_inside.
-    simpl.
-    doOne ltac:(drop_constraints)
-                 drop_constraints_drill ltac:(repeat subst_refine_evar; cbv beta; simpl; try finish honing).
-    doOne ltac:(drop_constraints)
-                 drop_constraints_drill ltac:(repeat subst_refine_evar; cbv beta; simpl; try finish honing).
-    match type of H2 with
-    | context[ UnConstrQuery_In (qsSchema := ?schem) ?r_n ?R (fun r => Query_Where (@?P r) _)] =>
-      pose proof (@For_UnConstrQuery_In_Where_Prop schem R r_n P a2 _ H2); destruct a2;
-        simpl in *; try discriminate; inversion H7
-    end.
-    simpl in *; injection H4; intros; subst.
-    Local Transparent SumType.SumType_index.
-    Local Transparent SumType.inj_SumType.
-    compute in n; congruence.
-    Local Opaque SumType.SumType_index.
-    Local Opaque SumType.inj_SumType.
-    refine pick val _; eauto.
-    doOne ltac:(drop_constraints)
-                 drop_constraints_drill ltac:(repeat subst_refine_evar; cbv beta; simpl; try finish honing).
+    doOne implement_insert'''
+          ltac:(master_implement_drill
+          ltac:(CombineCase5 StringPrefixIndexUse EqIndexUse)
+          ltac:(CombineCase10 createEarlyStringPrefixTerm createEarlyEqualityTerm)
+          ltac:(CombineCase7 createLastStringPrefixTerm createLastEqualityTerm);
+                set_evars) ltac:(finish honing).
+    Time doOne implement_insert'''
+          ltac:(master_implement_drill
+          ltac:(CombineCase5 StringPrefixIndexUse EqIndexUse)
+          ltac:(CombineCase10 createEarlyStringPrefixTerm createEarlyEqualityTerm)
+          ltac:(CombineCase7 createLastStringPrefixTerm createLastEqualityTerm);
+                set_evars) ltac:(finish honing).
+    Time doOne implement_insert'''
+          ltac:(master_implement_drill
+          ltac:(CombineCase5 StringPrefixIndexUse EqIndexUse)
+          ltac:(CombineCase10 createEarlyStringPrefixTerm createEarlyEqualityTerm)
+          ltac:(CombineCase7 createLastStringPrefixTerm createLastEqualityTerm);
+                set_evars) ltac:(finish honing).
+    clear H1.
+    Time doOne implement_insert'''
+          ltac:(master_implement_drill
+          ltac:(CombineCase5 StringPrefixIndexUse EqIndexUse)
+          ltac:(CombineCase10 createEarlyStringPrefixTerm createEarlyEqualityTerm)
+          ltac:(CombineCase7 createLastStringPrefixTerm createLastEqualityTerm);
+                set_evars) ltac:(finish honing).
+    Time doOne implement_insert'''
+          ltac:(master_implement_drill
+          ltac:(CombineCase5 StringPrefixIndexUse EqIndexUse)
+          ltac:(CombineCase10 createEarlyStringPrefixTerm createEarlyEqualityTerm)
+          ltac:(CombineCase7 createLastStringPrefixTerm createLastEqualityTerm);
+                set_evars) ltac:(finish honing).
+    Time doOne implement_insert'''
+          ltac:(master_implement_drill
+          ltac:(CombineCase5 StringPrefixIndexUse EqIndexUse)
+          ltac:(CombineCase10 createEarlyStringPrefixTerm createEarlyEqualityTerm)
+          ltac:(CombineCase7 createLastStringPrefixTerm createLastEqualityTerm);
+                set_evars) ltac:(finish honing).
+    Time doOne implement_insert'''
+          ltac:(master_implement_drill
+          ltac:(CombineCase5 StringPrefixIndexUse EqIndexUse)
+          ltac:(CombineCase10 createEarlyStringPrefixTerm createEarlyEqualityTerm)
+          ltac:(CombineCase7 createLastStringPrefixTerm createLastEqualityTerm);
+                set_evars) ltac:(finish honing).
+    Time doOne implement_insert'''
+          ltac:(master_implement_drill
+          ltac:(CombineCase5 StringPrefixIndexUse EqIndexUse)
+          ltac:(CombineCase10 createEarlyStringPrefixTerm createEarlyEqualityTerm)
+          ltac:(CombineCase7 createLastStringPrefixTerm createLastEqualityTerm);
+                set_evars) ltac:(finish honing).
+    Time doOne implement_insert'''
+          ltac:(master_implement_drill
+          ltac:(CombineCase5 StringPrefixIndexUse EqIndexUse)
+          ltac:(CombineCase10 createEarlyStringPrefixTerm createEarlyEqualityTerm)
+          ltac:(CombineCase7 createLastStringPrefixTerm createLastEqualityTerm);
+                set_evars) ltac:(finish honing).
+    Time doOne implement_insert'''
+          ltac:(master_implement_drill
+          ltac:(CombineCase5 StringPrefixIndexUse EqIndexUse)
+          ltac:(CombineCase10 createEarlyStringPrefixTerm createEarlyEqualityTerm)
+          ltac:(CombineCase7 createLastStringPrefixTerm createLastEqualityTerm);
+                set_evars) ltac:(finish honing).
+    Time doOne implement_insert'''
+          ltac:(master_implement_drill
+          ltac:(CombineCase5 StringPrefixIndexUse EqIndexUse)
+          ltac:(CombineCase10 createEarlyStringPrefixTerm createEarlyEqualityTerm)
+          ltac:(CombineCase7 createLastStringPrefixTerm createLastEqualityTerm);
+                set_evars) ltac:(finish honing).
+    Time doOne implement_insert'''
+          ltac:(master_implement_drill
+          ltac:(CombineCase5 StringPrefixIndexUse EqIndexUse)
+          ltac:(CombineCase10 createEarlyStringPrefixTerm createEarlyEqualityTerm)
+          ltac:(CombineCase7 createLastStringPrefixTerm createLastEqualityTerm);
+                set_evars) ltac:(finish honing).
+    Time doOne implement_insert'''
+          ltac:(master_implement_drill
+          ltac:(CombineCase5 StringPrefixIndexUse EqIndexUse)
+          ltac:(CombineCase10 createEarlyStringPrefixTerm createEarlyEqualityTerm)
+          ltac:(CombineCase7 createLastStringPrefixTerm createLastEqualityTerm);
+                set_evars) ltac:(finish honing).
+    Time doOne implement_insert'''
+          ltac:(master_implement_drill
+          ltac:(CombineCase5 StringPrefixIndexUse EqIndexUse)
+          ltac:(CombineCase10 createEarlyStringPrefixTerm createEarlyEqualityTerm)
+          ltac:(CombineCase7 createLastStringPrefixTerm createLastEqualityTerm);
+                set_evars) ltac:(finish honing).
+    Time doOne implement_insert'''
+          ltac:(master_implement_drill
+          ltac:(CombineCase5 StringPrefixIndexUse EqIndexUse)
+          ltac:(CombineCase10 createEarlyStringPrefixTerm createEarlyEqualityTerm)
+          ltac:(CombineCase7 createLastStringPrefixTerm createLastEqualityTerm);
+                set_evars) ltac:(finish honing).
+    Time doOne implement_insert'''
+          ltac:(master_implement_drill
+          ltac:(CombineCase5 StringPrefixIndexUse EqIndexUse)
+          ltac:(CombineCase10 createEarlyStringPrefixTerm createEarlyEqualityTerm)
+          ltac:(CombineCase7 createLastStringPrefixTerm createLastEqualityTerm);
+                set_evars) ltac:(finish honing).
+    Time doOne implement_insert'''
+          ltac:(master_implement_drill
+          ltac:(CombineCase5 StringPrefixIndexUse EqIndexUse)
+          ltac:(CombineCase10 createEarlyStringPrefixTerm createEarlyEqualityTerm)
+          ltac:(CombineCase7 createLastStringPrefixTerm createLastEqualityTerm);
+                set_evars) ltac:(finish honing).
+    Time doOne implement_insert'''
+          ltac:(master_implement_drill
+          ltac:(CombineCase5 StringPrefixIndexUse EqIndexUse)
+          ltac:(CombineCase10 createEarlyStringPrefixTerm createEarlyEqualityTerm)
+          ltac:(CombineCase7 createLastStringPrefixTerm createLastEqualityTerm);
+                set_evars) ltac:(finish honing).
 
-    doOne ltac:(drop_constraints)
-                 drop_constraints_drill ltac:(repeat subst_refine_evar; cbv beta; simpl; try finish honing).
-    doOne ltac:(drop_constraints)
-                 drop_constraints_drill ltac:(repeat subst_refine_evar; cbv beta; simpl; try finish honing).
-    doOne ltac:(drop_constraints)
-                 drop_constraints_drill ltac:(repeat subst_refine_evar; cbv beta; simpl; try finish honing).
-    setoid_rewrite refine_If_Then_Bind.
-    rewrite refine_Process_Query_Exact_Match by eassumption.
-    doOne ltac:(drop_constraints)
-                 drop_constraints_drill ltac:(repeat subst_refine_evar; cbv beta; simpl; try finish honing).
-    doOne ltac:(drop_constraints)
-                 drop_constraints_drill ltac:(repeat subst_refine_evar; cbv beta; simpl; try finish honing).
-    rewrite refine_For_List.
-    rewrite (refine_Iterate_Equiv_QueryResultComp _ H0).
-    repeat subst_refine_evar; cbv beta; simpl; try finish honing.
-    doOne ltac:(drop_constraints)
-                 drop_constraints_drill ltac:(repeat subst_refine_evar; cbv beta; simpl; try finish honing).
-    doOne ltac:(drop_constraints)
-                 drop_constraints_drill ltac:(repeat subst_refine_evar; cbv beta; simpl; try finish honing).
-    etransitivity; set_refine_evar.
-    doOne ltac:(drop_constraints)
-                 drop_constraints_drill ltac:(repeat subst_refine_evar; cbv beta; simpl; try finish honing).
-    etransitivity.
-    apply refine_MaxElements'.
-    rewrite (refine_QueryIn_Where _ _ H0).
-    rewrite (UnConstrQuery_In_Where_Map).
-
-    rewrite refine_For_Bind.
-    finish honing.
-
-    rewrite refine_MaxElements_map.
-    finish honing.
-    finish honing.
-    simplify with monad laws.
-
-    doOne ltac:(drop_constraints)
-                 drop_constraints_drill ltac:(repeat subst_refine_evar; cbv beta; simpl; try finish honing).
-    repeat doOne ltac:(drop_constraints)
-                 drop_constraints_drill ltac:(repeat subst_refine_evar; cbv beta; simpl; try finish honing).
-    rewrite refine_filter_Tuple_Decompose_inj'.
-    simplify with monad laws.
-    doOne ltac:(drop_constraints)
-                 drop_constraints_drill ltac:(repeat subst_refine_evar; cbv beta; simpl; try finish honing).
-    doOne ltac:(drop_constraints)
-                 drop_constraints_drill ltac:(repeat subst_refine_evar; cbv beta; simpl; try finish honing).
-    doOne ltac:(drop_constraints)
-                 drop_constraints_drill ltac:(repeat subst_refine_evar; cbv beta; simpl; try finish honing).
+   Time doOne implement_insert'''
+          ltac:(master_implement_drill
+          ltac:(CombineCase5 StringPrefixIndexUse EqIndexUse)
+          ltac:(CombineCase10 createEarlyStringPrefixTerm createEarlyEqualityTerm)
+          ltac:(CombineCase7 createLastStringPrefixTerm createLastEqualityTerm);
+                set_evars) ltac:(finish honing).
+    Time doOne implement_insert'''
+          ltac:(master_implement_drill
+          ltac:(CombineCase5 StringPrefixIndexUse EqIndexUse)
+          ltac:(CombineCase10 createEarlyStringPrefixTerm createEarlyEqualityTerm)
+          ltac:(CombineCase7 createLastStringPrefixTerm createLastEqualityTerm);
+                set_evars) ltac:(finish honing).
+    Time doOne implement_insert'''
+          ltac:(master_implement_drill
+          ltac:(CombineCase5 StringPrefixIndexUse EqIndexUse)
+          ltac:(CombineCase10 createEarlyStringPrefixTerm createEarlyEqualityTerm)
+          ltac:(CombineCase7 createLastStringPrefixTerm createLastEqualityTerm);
+                set_evars) ltac:(finish honing).
+    Time doOne implement_insert'''
+          ltac:(master_implement_drill
+          ltac:(CombineCase5 StringPrefixIndexUse EqIndexUse)
+          ltac:(CombineCase10 createEarlyStringPrefixTerm createEarlyEqualityTerm)
+          ltac:(CombineCase7 createLastStringPrefixTerm createLastEqualityTerm);
+                set_evars) ltac:(finish honing).
+    Time doOne implement_insert'''
+          ltac:(master_implement_drill
+          ltac:(CombineCase5 StringPrefixIndexUse EqIndexUse)
+          ltac:(CombineCase10 createEarlyStringPrefixTerm createEarlyEqualityTerm)
+          ltac:(CombineCase7 createLastStringPrefixTerm createLastEqualityTerm);
+                set_evars) ltac:(finish honing).
+    Time doOne implement_insert'''
+          ltac:(master_implement_drill
+          ltac:(CombineCase5 StringPrefixIndexUse EqIndexUse)
+          ltac:(CombineCase10 createEarlyStringPrefixTerm createEarlyEqualityTerm)
+          ltac:(CombineCase7 createLastStringPrefixTerm createLastEqualityTerm);
+                set_evars) ltac:(finish honing).
+    Time doOne implement_insert'''
+          ltac:(master_implement_drill
+          ltac:(CombineCase5 StringPrefixIndexUse EqIndexUse)
+          ltac:(CombineCase10 createEarlyStringPrefixTerm createEarlyEqualityTerm)
+          ltac:(CombineCase7 createLastStringPrefixTerm createLastEqualityTerm);
+                set_evars) ltac:(finish honing).
+    Time doOne implement_insert'''
+          ltac:(master_implement_drill
+          ltac:(CombineCase5 StringPrefixIndexUse EqIndexUse)
+          ltac:(CombineCase10 createEarlyStringPrefixTerm createEarlyEqualityTerm)
+          ltac:(CombineCase7 createLastStringPrefixTerm createLastEqualityTerm);
+                set_evars) ltac:(finish honing).
+    Time doOne implement_insert'''
+          ltac:(master_implement_drill
+          ltac:(CombineCase5 StringPrefixIndexUse EqIndexUse)
+          ltac:(CombineCase10 createEarlyStringPrefixTerm createEarlyEqualityTerm)
+          ltac:(CombineCase7 createLastStringPrefixTerm createLastEqualityTerm);
+                set_evars) ltac:(finish honing).
+    Time doOne implement_insert'''
+          ltac:(master_implement_drill
+          ltac:(CombineCase5 StringPrefixIndexUse EqIndexUse)
+          ltac:(CombineCase10 createEarlyStringPrefixTerm createEarlyEqualityTerm)
+          ltac:(CombineCase7 createLastStringPrefixTerm createLastEqualityTerm);
+                set_evars) ltac:(finish honing).
+    Time doOne implement_insert'''
+          ltac:(master_implement_drill
+          ltac:(CombineCase5 StringPrefixIndexUse EqIndexUse)
+          ltac:(CombineCase10 createEarlyStringPrefixTerm createEarlyEqualityTerm)
+          ltac:(CombineCase7 createLastStringPrefixTerm createLastEqualityTerm);
+                set_evars) ltac:(finish honing).
+    Time doOne implement_insert'''
+          ltac:(master_implement_drill
+          ltac:(CombineCase5 StringPrefixIndexUse EqIndexUse)
+          ltac:(CombineCase10 createEarlyStringPrefixTerm createEarlyEqualityTerm)
+          ltac:(CombineCase7 createLastStringPrefixTerm createLastEqualityTerm);
+                set_evars) ltac:(finish honing).
+    Time doOne implement_insert'''
+          ltac:(master_implement_drill
+          ltac:(CombineCase5 StringPrefixIndexUse EqIndexUse)
+          ltac:(CombineCase10 createEarlyStringPrefixTerm createEarlyEqualityTerm)
+          ltac:(CombineCase7 createLastStringPrefixTerm createLastEqualityTerm);
+                set_evars) ltac:(finish honing).
+    rewrite refine_MaxPrefix.
+    Time doOne implement_insert'''
+          ltac:(master_implement_drill
+          ltac:(CombineCase5 StringPrefixIndexUse EqIndexUse)
+          ltac:(CombineCase10 createEarlyStringPrefixTerm createEarlyEqualityTerm)
+          ltac:(CombineCase7 createLastStringPrefixTerm createLastEqualityTerm);
+                set_evars) ltac:(finish honing).
+    Time doOne implement_insert'''
+          ltac:(master_implement_drill
+          ltac:(CombineCase5 StringPrefixIndexUse EqIndexUse)
+          ltac:(CombineCase10 createEarlyStringPrefixTerm createEarlyEqualityTerm)
+          ltac:(CombineCase7 createLastStringPrefixTerm createLastEqualityTerm);
+                set_evars) ltac:(finish honing).
+    Time doOne implement_insert'''
+          ltac:(master_implement_drill
+          ltac:(CombineCase5 StringPrefixIndexUse EqIndexUse)
+          ltac:(CombineCase10 createEarlyStringPrefixTerm createEarlyEqualityTerm)
+          ltac:(CombineCase7 createLastStringPrefixTerm createLastEqualityTerm);
+                set_evars) ltac:(finish honing).
+    Time doOne implement_insert'''
+          ltac:(master_implement_drill
+          ltac:(CombineCase5 StringPrefixIndexUse EqIndexUse)
+          ltac:(CombineCase10 createEarlyStringPrefixTerm createEarlyEqualityTerm)
+          ltac:(CombineCase7 createLastStringPrefixTerm createLastEqualityTerm);
+                set_evars) ltac:(finish honing).
+   Time doOne implement_insert'''
+          ltac:(master_implement_drill
+          ltac:(CombineCase5 StringPrefixIndexUse EqIndexUse)
+          ltac:(CombineCase10 createEarlyStringPrefixTerm createEarlyEqualityTerm)
+          ltac:(CombineCase7 createLastStringPrefixTerm createLastEqualityTerm);
+                set_evars) ltac:(finish honing).
+    Time doOne implement_insert'''
+          ltac:(master_implement_drill
+          ltac:(CombineCase5 StringPrefixIndexUse EqIndexUse)
+          ltac:(CombineCase10 createEarlyStringPrefixTerm createEarlyEqualityTerm)
+          ltac:(CombineCase7 createLastStringPrefixTerm createLastEqualityTerm);
+                set_evars) ltac:(finish honing).
+    Time doOne implement_insert'''
+          ltac:(master_implement_drill
+          ltac:(CombineCase5 StringPrefixIndexUse EqIndexUse)
+          ltac:(CombineCase10 createEarlyStringPrefixTerm createEarlyEqualityTerm)
+          ltac:(CombineCase7 createLastStringPrefixTerm createLastEqualityTerm);
+                set_evars) ltac:(finish honing).
+    Time doOne implement_insert'''
+          ltac:(master_implement_drill
+          ltac:(CombineCase5 StringPrefixIndexUse EqIndexUse)
+          ltac:(CombineCase10 createEarlyStringPrefixTerm createEarlyEqualityTerm)
+          ltac:(CombineCase7 createLastStringPrefixTerm createLastEqualityTerm);
+                set_evars) ltac:(finish honing).
     apply refine_foldComp; intros ? ?; set_refine_evar.
-    rewrite (refine_Iterate_Equiv_QueryResultComp _ H0).
-    Local Opaque Query_For.
-    doOne ltac:(drop_constraints)
-                 drop_constraints_drill ltac:(repeat subst_refine_evar; cbv beta; simpl; try finish honing).
-    doOne ltac:(drop_constraints)
-                 drop_constraints_drill ltac:(repeat subst_refine_evar; cbv beta; simpl; try finish honing).
-    doOne ltac:(drop_constraints)
-                 drop_constraints_drill ltac:(repeat subst_refine_evar; cbv beta; simpl; try finish honing).
-    doOne ltac:(drop_constraints)
-                 drop_constraints_drill ltac:(repeat subst_refine_evar; cbv beta; simpl; try finish honing).
-    doOne ltac:(drop_constraints)
-                 drop_constraints_drill ltac:(repeat subst_refine_evar; cbv beta; simpl; try finish honing).
-    doOne ltac:(drop_constraints)
-                 drop_constraints_drill ltac:(repeat subst_refine_evar; cbv beta; simpl; try finish honing).
-    rewrite (refine_QueryIn_Where _ _ H0).
-    doOne ltac:(drop_constraints)
-                 drop_constraints_drill ltac:(repeat subst_refine_evar; cbv beta; simpl; try finish honing).
-    doOne ltac:(drop_constraints)
-                 drop_constraints_drill ltac:(repeat subst_refine_evar; cbv beta; simpl; try finish honing).
-    rewrite (refine_Iterate_Equiv_QueryResultComp _ H0).
-    doOne ltac:(drop_constraints)
-                 drop_constraints_drill ltac:(repeat subst_refine_evar; cbv beta; simpl; try finish honing).
-    doOne ltac:(drop_constraints)
-                 drop_constraints_drill ltac:(repeat subst_refine_evar; cbv beta; simpl; try finish honing).
-    doOne ltac:(drop_constraints)
-                 drop_constraints_drill ltac:(repeat subst_refine_evar; cbv beta; simpl; try finish honing).
-    etransitivity.
-    doOne ltac:(drop_constraints)
-                 drop_constraints_drill ltac:(repeat subst_refine_evar; cbv beta; simpl; try finish honing).
-    doOne ltac:(drop_constraints)
-                 drop_constraints_drill ltac:(repeat subst_refine_evar; cbv beta; simpl; try finish honing).
-    rewrite (refine_QueryIn_Where _ _ H0).
-    rewrite (UnConstrQuery_In_Where_Map).
-    rewrite refine_For_Bind.
-    finish honing.
-    finish honing.
-    rewrite refine_MaxElements_map.
-    simplify with monad laws.
-    doOne ltac:(drop_constraints)
-                 drop_constraints_drill ltac:(repeat subst_refine_evar; cbv beta; simpl; try finish honing).
-    repeat doOne ltac:(drop_constraints)
-                 drop_constraints_drill ltac:(repeat subst_refine_evar; cbv beta; simpl; try finish honing).
-    rewrite refine_filter_Tuple_Decompose_inj'.
-    simplify with monad laws.
-    doOne ltac:(drop_constraints)
-                 drop_constraints_drill ltac:(repeat subst_refine_evar; cbv beta; simpl; try finish honing).
-    doOne ltac:(drop_constraints)
-                 drop_constraints_drill ltac:(repeat subst_refine_evar; cbv beta; simpl; try finish honing).
-    doOne ltac:(drop_constraints)
-                 drop_constraints_drill ltac:(repeat subst_refine_evar; cbv beta; simpl; try finish honing).
-    apply refine_foldComp; intros ? ?; set_refine_evar.
-    rewrite (refine_Iterate_Equiv_QueryResultComp _ H0).
-    doOne ltac:(drop_constraints)
-                 drop_constraints_drill ltac:(repeat subst_refine_evar; cbv beta; simpl; try finish honing).
-    doOne ltac:(drop_constraints)
-                 drop_constraints_drill ltac:(repeat subst_refine_evar; cbv beta; simpl; try finish honing).
-    doOne ltac:(drop_constraints)
-                 drop_constraints_drill ltac:(repeat subst_refine_evar; cbv beta; simpl; try finish honing).
-    doOne ltac:(drop_constraints)
-                 drop_constraints_drill ltac:(repeat subst_refine_evar; cbv beta; simpl; try finish honing).
-    etransitivity.
-    doOne ltac:(drop_constraints)
-                 drop_constraints_drill ltac:(repeat subst_refine_evar; cbv beta; simpl; try finish honing).
-    apply refine_MaxElements'.
-    rewrite (refine_QueryIn_Where _ _ H0).
-    rewrite (UnConstrQuery_In_Where_Map).
-    rewrite refine_For_Bind.
-    finish honing.
-    finish honing.
-    rewrite refine_MaxElements_map.
-    simplify with monad laws.
-    doOne ltac:(drop_constraints)
-                 drop_constraints_drill ltac:(repeat subst_refine_evar; cbv beta; simpl; try finish honing).
-    repeat doOne ltac:(drop_constraints)
-                 drop_constraints_drill ltac:(repeat subst_refine_evar; cbv beta; simpl; try finish honing).
-    rewrite refine_filter_Tuple_Decompose_inj'.
-    simplify with monad laws.
-    doOne ltac:(drop_constraints)
-                 drop_constraints_drill ltac:(repeat subst_refine_evar; cbv beta; simpl; try finish honing).
-    doOne ltac:(drop_constraints)
-                 drop_constraints_drill ltac:(repeat subst_refine_evar; cbv beta; simpl; try finish honing).
-    doOne ltac:(drop_constraints)
-                 drop_constraints_drill ltac:(repeat subst_refine_evar; cbv beta; simpl; try finish honing).
-    apply refine_foldComp; intros ? ?; set_refine_evar.
-    rewrite (refine_Iterate_Equiv_QueryResultComp _ H0).
-
-    doOne ltac:(drop_constraints)
-                 drop_constraints_drill ltac:(repeat subst_refine_evar; cbv beta; simpl; try finish honing).
-    doOne ltac:(drop_constraints)
-                 drop_constraints_drill ltac:(repeat subst_refine_evar; cbv beta; simpl; try finish honing).
-    doOne ltac:(drop_constraints)
-                 drop_constraints_drill ltac:(repeat subst_refine_evar; cbv beta; simpl; try finish honing).
-    doOne ltac:(drop_constraints)
-                 drop_constraints_drill ltac:(repeat subst_refine_evar; cbv beta; simpl; try finish honing).
-    simpl.
-    finish honing.
-    repeat doOne ltac:(drop_constraints)
-                 drop_constraints_drill ltac:(repeat subst_refine_evar; cbv beta; simpl; try finish honing).
-    refine pick val _; eauto; finish honing.
-    repeat doOne ltac:(drop_constraints)
-                 drop_constraints_drill ltac:(repeat subst_refine_evar; cbv beta; simpl; try finish honing).
-    refine pick val _; eauto; finish honing.
-  }
-
-  { simplify with monad laws.
-    rewrite  refine_decode_packet.
-    doAny implement_insert''
-          ltac:(master_implement_drill EqIndexUse createEarlyEqualityTerm createLastEqualityTerm; set_evars) ltac:(finish honing).
-  }
-  + hone method "AddData".
-    subst.
-    simpl.
-    doAny ltac:(first [rewrite refine_bind_bind
-                      | rewrite refine_bind_unit
-                      | rewrite refineEquiv_pick_eq'
-                      | simplify with monad laws])
-                 ltac:(master_implement_drill EqIndexUse createEarlyEqualityTerm createLastEqualityTerm; set_evars; simpl) ltac:(finish honing).
-    simpl.
-    apply reflexivityT.
-
-  start sharpening ADT; unfold DnsSpec.
-  pose_string_hyps; pose_heading_hyps.
-  drop_constraintsfrom_DNS.
-  { (* Add Data. *)
-    match goal with
-      H : DropQSConstraints_AbsR ?r_o ?r_n
-      |- refine (u <- QSInsert ?r_o ?Ridx ?tup;
-                 @?k u) _ =>
-      eapply (@QSInsertSpec_refine_subgoals _ _ r_o r_n Ridx tup); try exact H
-    end; try set_refine_evar.
-    - rewrite decides_True; finish honing.
-    - simpl.
-
-rewrite refine_decides_forall_and;
-  [
-  | let a := fresh in
-   intro a; split; [let H' := fresh in intros H'; pattern (indexedElement a); exact H' | intuition]
-  | let a := fresh in
-    intro a; split; [let H' := fresh in intros H'; pattern (indexedElement a); exact H' | intuition] ].
-      rewrite refine_noDup_CNAME_check_dns by eauto.
-    doOne ltac:(drop_constraints)
-                 drop_constraints_drill ltac:(repeat subst_refine_evar; cbv beta; simpl; try finish honing).
-    match goal with
-      |- refine (If_Then_Else ?c _ _) _ =>
-      subst_refine_evar; eapply refine_if with (b := c);
-        let H := fresh in
-        intro H; set_refine_evar; try rewrite H; simpl
-    end.
-    doOne ltac:(drop_constraints)
-                 drop_constraints_drill ltac:(repeat subst_refine_evar; cbv beta; simpl; try finish honing).
-    doOne ltac:(drop_constraints)
-                 drop_constraints_drill ltac:(repeat subst_refine_evar; cbv beta; simpl; try finish honing).
-    doOne ltac:(drop_constraints)
-                 drop_constraints_drill ltac:(repeat subst_refine_evar; cbv beta; simpl; try finish honing).
-    doOne ltac:(drop_constraints)
-                 drop_constraints_drill ltac:(repeat subst_refine_evar; cbv beta; simpl; try finish honing).
-    rewrite refine_no_usurp_authority_check by eauto.
-    erewrite beq_RRecordType_trans by eauto.
-    simpl.
-    doOne ltac:(drop_constraints)
-                 drop_constraints_drill ltac:(repeat subst_refine_evar; cbv beta; simpl; try finish honing).
-    doOne ltac:(drop_constraints)
-                 drop_constraints_drill ltac:(repeat subst_refine_evar; cbv beta; simpl; try finish honing).
-    doOne ltac:(drop_constraints)
-                 drop_constraints_drill ltac:(repeat subst_refine_evar; cbv beta; simpl; try finish honing).
-    doOne ltac:(drop_constraints)
-                 drop_constraints_drill ltac:(repeat subst_refine_evar; cbv beta; simpl; try finish honing).
-    rewrite refine_no_usurp_authority_check_dns by eauto.
-    repeat doOne ltac:(drop_constraints)
-                        drop_constraints_drill ltac:(repeat subst_refine_evar; cbv beta; simpl; try finish honing).
-    doOne ltac:(drop_constraints)
-                 drop_constraints_drill ltac:(repeat subst_refine_evar; cbv beta; simpl; try finish honing).
-    - simpl; set_evars; intros.
-      rewrite refine_decides_forall_and;
-        [
-        | let a := fresh in
-          intro a; split; [let H' := fresh in intros H'; pattern (indexedElement a); exact H' | intuition]
-        | let a := fresh in
-          intro a; split; [let H' := fresh in intros H'; pattern (indexedElement a); exact H' | intuition] ].
-      setoid_rewrite refine_count_constraint_broken'.
-      doOne ltac:(drop_constraints)
-                   drop_constraints_drill ltac:(repeat subst_refine_evar; cbv beta; simpl; try finish honing).
-      doOne ltac:(drop_constraints)
-                   drop_constraints_drill ltac:(repeat subst_refine_evar; cbv beta; simpl; try finish honing).
-      doOne ltac:(drop_constraints)
-                   drop_constraints_drill ltac:(repeat subst_refine_evar; cbv beta; simpl; try finish honing).
-      doOne ltac:(drop_constraints)
-                   drop_constraints_drill ltac:(repeat subst_refine_evar; cbv beta; simpl; try finish honing).
-      rewrite refine_no_usurp_authority_check'_dns by eauto.
-      repeat doOne ltac:(drop_constraints)
-                          drop_constraints_drill ltac:(repeat subst_refine_evar; cbv beta; simpl; try finish honing).
-      repeat doOne ltac:(drop_constraints)
-                          drop_constraints_drill ltac:(repeat subst_refine_evar; cbv beta; simpl; try finish honing).
-    - simpl; finish honing.
-    - simpl; intros; finish honing.
-    - intros. refine pick val _; eauto; simplify with monad laws.
-      simpl; finish honing.
-    - intros. refine pick val _; eauto; simplify with monad laws.
-      simpl; finish honing.
-  }
-  { (* Process *)
-    doOne ltac:(drop_constraints)
-                 drop_constraints_drill ltac:(repeat subst_refine_evar; cbv beta; simpl; try finish honing).
-    doOne ltac:(drop_constraints)
-                 drop_constraints_drill ltac:(repeat subst_refine_evar; cbv beta; simpl; try finish honing).
-    doOne ltac:(drop_constraints)
-                 drop_constraints_drill ltac:(repeat subst_refine_evar; cbv beta; simpl; try finish honing).
-    doOne ltac:(drop_constraints)
-                 drop_constraints_drill ltac:(repeat subst_refine_evar; cbv beta; simpl; try finish honing).
-    doOne ltac:(drop_constraints)
-                 drop_constraints_drill ltac:(repeat subst_refine_evar; cbv beta; simpl; try finish honing).
-    doOne ltac:(drop_constraints)
-                 drop_constraints_drill ltac:(repeat subst_refine_evar; cbv beta; simpl; try finish honing).
-    doOne ltac:(drop_constraints)
-                 drop_constraints_drill ltac:(repeat subst_refine_evar; cbv beta; simpl; try finish honing).
-    doOne ltac:(drop_constraints)
-                 drop_constraints_drill ltac:(repeat subst_refine_evar; cbv beta; simpl; try finish honing).
-    doOne ltac:(drop_constraints)
-                 drop_constraints_drill ltac:(repeat subst_refine_evar; cbv beta; simpl; try finish honing).
-    etransitivity.
-    doOne ltac:(drop_constraints)
-                 drop_constraints_drill ltac:(repeat subst_refine_evar; cbv beta; simpl; try finish honing).
-    etransitivity.
-    doOne ltac:(drop_constraints)
-                 drop_constraints_drill ltac:(repeat subst_refine_evar; cbv beta; simpl; try finish honing).
-    doOne ltac:(drop_constraints)
-                 drop_constraints_drill ltac:(repeat subst_refine_evar; cbv beta; simpl; try finish honing).
-    doOne ltac:(drop_constraints)
-                 drop_constraints_drill ltac:(repeat subst_refine_evar; cbv beta; simpl; try finish honing).
-    rewrite (@MaxElementsUnConstrQuery_In DnsSchema Fin.F1 (fun r : resourceRecord => GetAttributeRaw r Fin.F1) a1 r_n).
-    rewrite refine_Process_Query.
-    simplify with monad laws.
-    setoid_rewrite refine_If_Opt_Then_Else_Bind.
-    setoid_rewrite refineEquiv_bind_unit; simpl.
-    finish honing.
-    eassumption.
-    finish honing.
-    set_refine_evar; simpl.
-    doOne ltac:(drop_constraints)
-                 drop_constraints_drill ltac:(repeat subst_refine_evar; cbv beta; simpl; try finish honing).
-    doOne ltac:(drop_constraints)
-                 drop_constraints_drill ltac:(repeat subst_refine_evar; cbv beta; simpl; try finish honing).
-    doOne ltac:(drop_constraints)
-                 drop_constraints_drill ltac:(repeat subst_refine_evar; cbv beta; simpl; try finish honing).
-    rewrite refine_If_Opt_Then_Else_Bind.
-    unfold H3. eapply refine_If_Opt_Then_Else'; intros; set_refine_evar.
-    simplify with monad laws; simpl.
-    rewrite refine_IfDec_true.
-    simpl.
-    rewrite (fun q => @refine_Singleton_Set'' r_o _ q _ _ _ H2 H4).
-
-    doOne ltac:(drop_constraints)
-                 drop_constraints_drill ltac:(repeat subst_refine_evar; cbv beta; simpl; try finish honing).
-    doOne ltac:(drop_constraints)
-                 drop_constraints_drill ltac:(repeat subst_refine_evar; cbv beta; simpl; try finish honing).
-    doOne ltac:(drop_constraints)
-                 drop_constraints_drill ltac:(repeat subst_refine_evar; cbv beta; simpl; try finish honing).
-    doOne ltac:(drop_constraints)
-                 drop_constraints_drill ltac:(repeat subst_refine_evar; cbv beta; simpl; try finish honing).
-    doOne ltac:(drop_constraints)
-                 drop_constraints_drill ltac:(repeat subst_refine_evar; cbv beta; simpl; try finish honing).
-    doOne ltac:(drop_constraints)
-                 drop_constraints_drill ltac:(repeat subst_refine_evar; cbv beta; simpl; try finish honing).
-    doOne ltac:(drop_constraints)
-                 drop_constraints_drill ltac:(repeat subst_refine_evar; cbv beta; simpl; try finish honing).
-    doOne ltac:(drop_constraints)
-                 drop_constraints_drill ltac:(repeat subst_refine_evar; cbv beta; simpl; try finish honing).
-    doOne ltac:(drop_constraints)
-                 drop_constraints_drill ltac:(repeat subst_refine_evar; cbv beta; simpl; try finish honing).
-    doOne ltac:(drop_constraints)
-                 drop_constraints_drill ltac:(repeat subst_refine_evar; cbv beta; simpl; try finish honing).
-    doOne ltac:(drop_constraints)
-                 drop_constraints_drill ltac:(repeat subst_refine_evar; cbv beta; simpl; try finish honing).
-    doOne ltac:(drop_constraints)
-                 drop_constraints_drill ltac:(repeat subst_refine_evar; cbv beta; simpl; try finish honing).
-    doOne ltac:(drop_constraints)
-                 drop_constraints_drill ltac:(repeat subst_refine_evar; cbv beta; simpl; try finish honing).
-    doOne ltac:(drop_constraints)
-                 drop_constraints_drill ltac:(repeat subst_refine_evar; cbv beta; simpl; try finish honing).
-    doOne ltac:(drop_constraints)
-                 drop_constraints_drill ltac:(repeat subst_refine_evar; cbv beta; simpl; try finish honing).
-    doOne ltac:(drop_constraints)
-                 drop_constraints_drill ltac:(repeat subst_refine_evar; cbv beta; simpl; try finish honing).
-    doOne ltac:(drop_constraints)
-                 drop_constraints_drill ltac:(repeat subst_refine_evar; cbv beta; simpl; try finish honing).
-    repeat econstructor.
-    match type of H2 with
-    | context[ UnConstrQuery_In (qsSchema := ?schem) ?r_n ?R _] =>
-      pose proof (@For_UnConstrQuery_In_Where_Prop schem R r_n (fun r => RDataTypeToRRecordType r!sRDATA = CNAME /\ GetAttributeRaw r Fin.F1 = a1) _ _ H2);
-        destruct a2; simpl in H4; try discriminate; injections;
-          inversion H6; subst; intuition
-    end.
-    doOne ltac:(drop_constraints)
-                 drop_constraints_drill ltac:(repeat subst_refine_evar; cbv beta; simpl; try finish honing).
-    doOne ltac:(drop_constraints)
-                 drop_constraints_drill ltac:(repeat subst_refine_evar; cbv beta; simpl; try finish honing).
-    doOne ltac:(drop_constraints)
-                 drop_constraints_drill ltac:(repeat subst_refine_evar; cbv beta; simpl; try finish honing).
-    doOne ltac:(drop_constraints)
-                 drop_constraints_drill ltac:(repeat subst_refine_evar; cbv beta; simpl; try finish honing).
-    match goal with
-      |- refine (If_Then_Else ?c _ _) _ =>
-      subst_refine_evar; eapply refine_if with (b := c);
-        let H := fresh in
-        intro H; set_refine_evar; try rewrite H; simpl
-    end.
-    doOne ltac:(drop_constraints)
-                 drop_constraints_drill ltac:(repeat subst_refine_evar; cbv beta; simpl; try finish honing).
-    rewrite refine_If_Then_Else_false.
-    rewrite refine_IfDec_true.
-    rewrite (fun q => @refine_Singleton_Set' r_n q _ _ H4).
-    doOne ltac:(drop_constraints)
-                 drop_constraints_drill ltac:(repeat subst_refine_evar; cbv beta; simpl; try finish honing).
-    doOne ltac:(drop_constraints)
-                 drop_constraints_drill ltac:(repeat subst_refine_evar; cbv beta; simpl; try finish honing).
-    doOne ltac:(drop_constraints)
-                 drop_constraints_drill ltac:(repeat subst_refine_evar; cbv beta; simpl; try finish honing).
-    doOne ltac:(drop_constraints)
-                 drop_constraints_drill ltac:(repeat subst_refine_evar; cbv beta; simpl; try finish honing).
-    apply (@For_UnConstrQuery_In_Where_Prop DnsSchema Fin.F1 r_n _ a3 _) in H4.
-    rewrite Forall_forall in *.
-    intros; eapply H4; eauto.
-    rewrite <- negb_true_iff; eassumption.
-    etransitivity; set_refine_evar.
-    doOne ltac:(drop_constraints)
-                 drop_constraints_drill ltac:(repeat subst_refine_evar; cbv beta; simpl; try finish honing).
-    repeat doOne ltac:(drop_constraints)
-                 drop_constraints_drill ltac:(repeat subst_refine_evar; cbv beta; simpl; try finish honing).
-    match goal with
-      |- refine (If_Then_Else ?c _ _) _ =>
-      subst_refine_evar; eapply refine_if with (b := c);
-        let H := fresh in
-        intro H; set_refine_evar; try rewrite H; simpl
-    end.
-    doOne ltac:(drop_constraints)
-                 drop_constraints_drill ltac:(repeat subst_refine_evar; cbv beta; simpl; try finish honing).
-    rewrite refine_IfDec_false.
-    drop_constraints_drill.
-    doOne ltac:(drop_constraints)
-                 drop_constraints_drill ltac:(repeat subst_refine_evar; cbv beta; simpl; try finish honing).
-    drop_constraints_drill.
-    apply refine_foldComp; intros ? ?; set_refine_evar.
-    repeat doOne ltac:(drop_constraints)
-                 drop_constraints_drill ltac:(repeat subst_refine_evar; cbv beta; simpl; try finish honing).
-    doOne ltac:(drop_constraints)
-                 drop_constraints_drill ltac:(repeat subst_refine_evar; cbv beta; simpl; try finish honing).
-
-    destruct a4; simpl in *; try discriminate.
-    intro.
-    apply (@MaxElements_UnConstrQuery_In_Where_Prop DnsSchema Fin.F1 r_n) in H7.
-    rewrite Forall_forall in *.
-    eapply H7; simpl; intuition.
-    apply DecideableEnsemble_And.
-    simpl.
-    setoid_rewrite refine_If_Else_Bind.
-
-    rewrite refine_Process_Query_Imprecise_Match by eauto.
-
-    repeat doOne ltac:(drop_constraints)
-                        drop_constraints_drill ltac:(repeat subst_refine_evar; cbv beta; simpl; try finish honing).
-    repeat doOne ltac:(drop_constraints)
-                 drop_constraints_drill ltac:(repeat subst_refine_evar; cbv beta; simpl; try finish honing).
-    repeat doOne ltac:(drop_constraints)
-                        drop_constraints_drill ltac:(repeat subst_refine_evar; cbv beta; simpl; try finish honing).
-
-    (* 51s with apply decomposition lemmas.*)
-    (* 73s with rewrite decomposition lemmas.*)
-  }
-  simpl.
-  assert (forall (r : UnConstrQueryStructure
-                        (DecomposeRawQueryStructureSchema DnsSchema Fin.F1
-                                                          (Fin.FS (Fin.FS (Fin.FS Fin.F1))) ResourceRecordTypeTypes)), True).
-  unfold DecomposeRawQueryStructureSchema, DecomposeSchema in *; simpl in *.
-  pose_heading_hyps; auto.
-  clear H.
-  hone representation using (fun r_o (r_n : UnConstrQueryStructure qs_schema) =>
-                               exists r_n',
-                               @DecomposeRawQueryStructureSchema_AbsR
-                                 _ DnsSchema Fin.F1 (Fin.FS (Fin.FS (Fin.FS (Fin.F1)))) _
-                                 (SumType.SumType_index ResourceRecordTypeTypes)
-                                 (SumType.SumType_proj ResourceRecordTypeTypes)
-                                 (SumType.inj_SumType ResourceRecordTypeTypes)
-                                 r_o (r_n', r_n)).
-  { simplify with monad laws.
-    refine pick val _.
-    2: eexists _; apply (@DecomposeRawQueryStructureSchema_empty_AbsR _ DnsSchema).
-    finish honing.
-  }
-  { destruct_ex; simplify with monad laws.
-    drop_constraints_drill.
-    rewrite (refine_UnConstrFreshIdx_DecomposeRawQueryStructureSchema_AbsR_Equiv H0).
-    simpl; finish honing.
-    doOne ltac:(drop_constraints)
-                 drop_constraints_drill ltac:(repeat subst_refine_evar; cbv beta; simpl; try finish honing).
-    doOne ltac:(drop_constraints)
-                 drop_constraints_drill ltac:(repeat subst_refine_evar; cbv beta; simpl; try finish honing).
-    doOne ltac:(drop_constraints)
-                 drop_constraints_drill ltac:(repeat subst_refine_evar; cbv beta; simpl; try finish honing).
-    doOne ltac:(drop_constraints)
-                 drop_constraints_drill ltac:(repeat subst_refine_evar; cbv beta; simpl; try finish honing).
-    doOne ltac:(drop_constraints)
-                 drop_constraints_drill ltac:(repeat subst_refine_evar; cbv beta; simpl; try finish honing).
-    setoid_rewrite (refine_Iterate_Equiv_QueryResultComp _ H0).
-    (* simpl; unfold Tuple_DecomposeRawQueryStructure_inj; simpl. *)
-    simpl; finish honing.
-    doOne ltac:(drop_constraints)
-                 drop_constraints_drill ltac:(repeat subst_refine_evar; cbv beta; simpl; try finish honing).
-    doOne ltac:(drop_constraints)
-                 drop_constraints_drill ltac:(repeat subst_refine_evar; cbv beta; simpl; try finish honing).
-    doOne ltac:(drop_constraints)
-                 drop_constraints_drill ltac:(repeat subst_refine_evar; cbv beta; simpl; try finish honing).
-    doOne ltac:(drop_constraints)
-                 drop_constraints_drill ltac:(repeat subst_refine_evar; cbv beta; simpl; try finish honing).
-    setoid_rewrite Query_Where_And_Sym.
-    setoid_rewrite (refine_QueryIn_Where _ _ H0).
-    unfold Tuple_DecomposeRawQueryStructure_inj'; simpl.
-    unfold GetAttribute, GetAttributeRaw at 2; simpl.
-    unfold ilist2_hd; simpl.
-    finish honing.
-    doOne ltac:(drop_constraints)
-                 drop_constraints_drill ltac:(repeat subst_refine_evar; cbv beta; simpl; try finish honing).
-    doOne ltac:(drop_constraints)
-                 drop_constraints_drill ltac:(repeat subst_refine_evar; cbv beta; simpl; try finish honing).
-    doOne ltac:(drop_constraints)
-                 drop_constraints_drill ltac:(repeat subst_refine_evar; cbv beta; simpl; try finish honing).
-    doOne ltac:(drop_constraints)
-                 drop_constraints_drill ltac:(repeat subst_refine_evar; cbv beta; simpl; try finish honing).
-    doOne ltac:(drop_constraints)
-                 drop_constraints_drill ltac:(repeat subst_refine_evar; cbv beta; simpl; try finish honing).
-    simpl.
-    erewrite (DecomposeRawQueryStructureSchema_UpdateUnConstrRelationInsertC_eq _ _ H0);
-      [ | eassumption | intros; set_refine_evar; refine pick val (snd r_n'); destruct r_n';
-                        try eauto;
-                        simplify with monad laws; simpl; try finish honing;
-                        unfold H5; instantiate (1 := fun z => ret (snd z, true)); reflexivity].
-    simpl.
-    Local Transparent UpdateUnConstrRelationInsertC.
-    unfold UpdateUnConstrRelationInsertC at 1.
-    doOne ltac:(drop_constraints)
-                 drop_constraints_drill ltac:(repeat subst_refine_evar; cbv beta; simpl; try finish honing).
-    doOne ltac:(drop_constraints)
-                 drop_constraints_drill ltac:(repeat subst_refine_evar; cbv beta; simpl; try finish honing).
-    doOne ltac:(drop_constraints)
-                 drop_constraints_drill ltac:(repeat subst_refine_evar; cbv beta; simpl; try finish honing).
-    doOne ltac:(drop_constraints)
-                 drop_constraints_drill ltac:(repeat subst_refine_evar; cbv beta; simpl; try finish honing).
-    setoid_rewrite (refine_QueryIn_Where _ _ H0).
-    unfold Tuple_DecomposeRawQueryStructure_inj'; simpl.
-    unfold GetAttribute, GetAttributeRaw at 1; simpl.
-    unfold GetAttribute, GetAttributeRaw at 2; simpl.
-    unfold ilist2_hd; simpl.
-    doOne ltac:(drop_constraints)
-                 drop_constraints_drill ltac:(repeat subst_refine_evar; cbv beta; simpl; try finish honing).
-    doOne ltac:(drop_constraints)
-                 drop_constraints_drill ltac:(repeat subst_refine_evar; cbv beta; simpl; try finish honing).
-    simpl. finish honing.
-    rewrite !refine_if_If.
-    doOne ltac:(drop_constraints)
-                 drop_constraints_drill ltac:(repeat subst_refine_evar; cbv beta; simpl; try finish honing).
-    doOne ltac:(drop_constraints)
-                 drop_constraints_drill ltac:(repeat subst_refine_evar; cbv beta; simpl; try finish honing).
-    doOne ltac:(drop_constraints)
-                 drop_constraints_drill ltac:(repeat subst_refine_evar; cbv beta; simpl; try finish honing).
-    erewrite (DecomposeRawQueryStructureSchema_UpdateUnConstrRelationInsertC_eq _ _ H0);
-      [ | eassumption | intros; set_refine_evar; refine pick val (snd r_n'); destruct r_n';
-                        try eauto;
-                        simplify with monad laws; simpl; try finish honing;
-                        unfold H6; instantiate (1 := fun z => ret (snd z, true)); reflexivity].
-    simpl.
-    unfold UpdateUnConstrRelationInsertC at 1.
-    repeat doOne ltac:(drop_constraints)
-                        drop_constraints_drill ltac:(repeat subst_refine_evar; cbv beta; simpl; try finish honing).
-    repeat doOne ltac:(drop_constraints)
-                        drop_constraints_drill ltac:(repeat subst_refine_evar; cbv beta; simpl; try finish honing).
-    refine pick val _; eauto; finish honing.
-    repeat doOne ltac:(drop_constraints)
-                 drop_constraints_drill ltac:(repeat subst_refine_evar; cbv beta; simpl; try finish honing).
-    refine pick val _; eauto; finish honing.
-    doOne ltac:(drop_constraints)
-                 drop_constraints_drill ltac:(repeat subst_refine_evar; cbv beta; simpl; try finish honing).
-    doOne ltac:(drop_constraints)
-                 drop_constraints_drill ltac:(repeat subst_refine_evar; cbv beta; simpl; try finish honing).
-    setoid_rewrite Query_Where_And_Sym.
-    setoid_rewrite (refine_QueryIn_Where _ _ H0).
-    unfold Tuple_DecomposeRawQueryStructure_inj'; simpl.
-    unfold GetAttribute, GetAttributeRaw at 2; simpl.
-    unfold ilist2_hd; simpl.
-    finish honing.
-    repeat doOne ltac:(drop_constraints)
-                 drop_constraints_drill ltac:(repeat subst_refine_evar; cbv beta; simpl; try finish honing).
-    refine pick val _; eauto; finish honing.
-    setoid_rewrite (refine_QueryIn_Where _ _ H0).
-    unfold Tuple_DecomposeRawQueryStructure_inj'; simpl.
-    unfold GetAttribute, GetAttributeRaw at 1; simpl.
-    unfold GetAttribute, GetAttributeRaw at 2; simpl.
-    unfold ilist2_hd; simpl.
-    finish honing.
-    refine pick val _; eauto; finish honing.
-    refine pick val _; eauto; finish honing.
-    doOne ltac:(drop_constraints)
-                 drop_constraints_drill ltac:(repeat subst_refine_evar; cbv beta; simpl; try finish honing).
-    doOne ltac:(drop_constraints)
-                 drop_constraints_drill ltac:(repeat subst_refine_evar; cbv beta; simpl; try finish honing).
-    doOne ltac:(drop_constraints)
-                 drop_constraints_drill ltac:(repeat subst_refine_evar; cbv beta; simpl; try finish honing).
-    rewrite (refine_Iterate_Equiv_QueryResultComp _ H0).
-    doOne ltac:(drop_constraints)
-                 drop_constraints_drill ltac:(repeat subst_refine_evar; cbv beta; simpl; try finish honing).
-    doOne ltac:(drop_constraints)
-                 drop_constraints_drill ltac:(repeat subst_refine_evar; cbv beta; simpl; try finish honing).
-    setoid_rewrite Query_Where_And_Sym.
-    setoid_rewrite (refine_QueryIn_Where _ _ H0).
-    unfold Tuple_DecomposeRawQueryStructure_inj'; simpl.
-    unfold GetAttribute, GetAttributeRaw at 2; simpl.
-    unfold ilist2_hd; simpl.
-    finish honing.
-    doOne ltac:(drop_constraints)
-                 drop_constraints_drill ltac:(repeat subst_refine_evar; cbv beta; simpl; try finish honing).
-    doOne ltac:(drop_constraints)
-                 drop_constraints_drill ltac:(repeat subst_refine_evar; cbv beta; simpl; try finish honing).
-    doOne ltac:(drop_constraints)
-                 drop_constraints_drill ltac:(repeat subst_refine_evar; cbv beta; simpl; try finish honing).
-    doOne ltac:(drop_constraints)
-                 drop_constraints_drill ltac:(repeat subst_refine_evar; cbv beta; simpl; try finish honing).
-    doOne ltac:(drop_constraints)
-                 drop_constraints_drill ltac:(repeat subst_refine_evar; cbv beta; simpl; try finish honing).
-    rewrite refine_if_If.
-    doOne ltac:(drop_constraints)
-                 drop_constraints_drill ltac:(repeat subst_refine_evar; cbv beta; simpl; try finish honing).
-    doOne ltac:(drop_constraints)
-                 drop_constraints_drill ltac:(repeat subst_refine_evar; cbv beta; simpl; try finish honing).
-    doOne ltac:(drop_constraints)
-                 drop_constraints_drill ltac:(repeat subst_refine_evar; cbv beta; simpl; try finish honing).
-    erewrite (DecomposeRawQueryStructureSchema_UpdateUnConstrRelationInsertC_eq _ _ H0);
-      [ | eassumption | intros; set_refine_evar; refine pick val (snd r_n'); destruct r_n';
-                        try eauto;
-                        simplify with monad laws; simpl; try finish honing;
-                        unfold H5; instantiate (1 := fun z => ret (snd z, true)); reflexivity].
-    simpl; unfold UpdateUnConstrRelationInsertC at 1.
-    doOne ltac:(drop_constraints)
-                 drop_constraints_drill ltac:(repeat subst_refine_evar; cbv beta; simpl; try finish honing).
-    repeat doOne ltac:(drop_constraints)
-                 drop_constraints_drill ltac:(repeat subst_refine_evar; cbv beta; simpl; try finish honing).
-    repeat doOne ltac:(drop_constraints)
-                 drop_constraints_drill ltac:(repeat subst_refine_evar; cbv beta; simpl; try finish honing).
-    refine pick val _; eauto; finish honing.
-    doOne ltac:(drop_constraints)
-                 drop_constraints_drill ltac:(repeat subst_refine_evar; cbv beta; simpl; try finish honing).
-    doOne ltac:(drop_constraints)
-                 drop_constraints_drill ltac:(repeat subst_refine_evar; cbv beta; simpl; try finish honing).
-    setoid_rewrite (refine_QueryIn_Where _ _ H0).
-    unfold Tuple_DecomposeRawQueryStructure_inj'; simpl.
-    unfold GetAttribute, GetAttributeRaw at 1; simpl.
-    unfold GetAttribute, GetAttributeRaw at 2; simpl.
-    unfold ilist2_hd; simpl.
-    finish honing.
-    rewrite !refine_if_If.
-    doOne ltac:(drop_constraints)
-                 drop_constraints_drill ltac:(repeat subst_refine_evar; cbv beta; simpl; try finish honing).
-    doOne ltac:(drop_constraints)
-                 drop_constraints_drill ltac:(repeat subst_refine_evar; cbv beta; simpl; try finish honing).
-    doOne ltac:(drop_constraints)
-                 drop_constraints_drill ltac:(repeat subst_refine_evar; cbv beta; simpl; try finish honing).
-    doOne ltac:(drop_constraints)
-                 drop_constraints_drill ltac:(repeat subst_refine_evar; cbv beta; simpl; try finish honing).
-    doOne ltac:(drop_constraints)
-                 drop_constraints_drill ltac:(repeat subst_refine_evar; cbv beta; simpl; try finish honing).
-    erewrite (DecomposeRawQueryStructureSchema_UpdateUnConstrRelationInsertC_eq _ _ H0);
-      [ | eassumption | intros; set_refine_evar; refine pick val (snd r_n'); destruct r_n';
-                        try eauto;
-                        simplify with monad laws; simpl; try finish honing;
-                        unfold H6; instantiate (1 := fun z => ret (snd z, true)); reflexivity].
-    simpl.
-    simpl; unfold UpdateUnConstrRelationInsertC at 1.
-    doOne ltac:(drop_constraints)
-                 drop_constraints_drill ltac:(repeat subst_refine_evar; cbv beta; simpl; try finish honing).
-    repeat doOne ltac:(drop_constraints)
-                        drop_constraints_drill ltac:(repeat subst_refine_evar; cbv beta; simpl; try finish honing).
-    repeat doOne ltac:(drop_constraints)
-                        drop_constraints_drill ltac:(repeat subst_refine_evar; cbv beta; simpl; try finish honing).
-    refine pick val _; eauto; finish honing.
-    repeat doOne ltac:(drop_constraints)
-                        drop_constraints_drill ltac:(repeat subst_refine_evar; cbv beta; simpl; try finish honing).
-    refine pick val _; eauto; finish honing.
-    doOne ltac:(drop_constraints)
-                        drop_constraints_drill ltac:(repeat subst_refine_evar; cbv beta; simpl; try finish honing).
-    rewrite !refine_if_If.
-    doOne ltac:(drop_constraints)
-                 drop_constraints_drill ltac:(repeat subst_refine_evar; cbv beta; simpl; try finish honing).
-    repeat doOne ltac:(drop_constraints)
-                 drop_constraints_drill ltac:(repeat subst_refine_evar; cbv beta; simpl; try finish honing).
-    refine pick val _; eauto; finish honing.
-    refine pick val _; eauto; finish honing.
-    doOne ltac:(drop_constraints)
-                 drop_constraints_drill ltac:(repeat subst_refine_evar; cbv beta; simpl; try finish honing).
-    doOne ltac:(drop_constraints)
-                 drop_constraints_drill ltac:(repeat subst_refine_evar; cbv beta; simpl; try finish honing).
-    setoid_rewrite Query_Where_And_Sym.
-    setoid_rewrite (refine_QueryIn_Where _ _ H0).
-    unfold Tuple_DecomposeRawQueryStructure_inj'; simpl.
-    unfold GetAttribute, GetAttributeRaw at 2; simpl.
-    unfold ilist2_hd; simpl.
-    finish honing.
-    doOne ltac:(drop_constraints)
-                 drop_constraints_drill ltac:(repeat subst_refine_evar; cbv beta; simpl; try finish honing).
-    doOne ltac:(drop_constraints)
-                 drop_constraints_drill ltac:(repeat subst_refine_evar; cbv beta; simpl; try finish honing).
-    doOne ltac:(drop_constraints)
-                 drop_constraints_drill ltac:(repeat subst_refine_evar; cbv beta; simpl; try finish honing).
-    doOne ltac:(drop_constraints)
-                 drop_constraints_drill ltac:(repeat subst_refine_evar; cbv beta; simpl; try finish honing).
-    doOne ltac:(drop_constraints)
-                 drop_constraints_drill ltac:(repeat subst_refine_evar; cbv beta; simpl; try finish honing).
-    erewrite (DecomposeRawQueryStructureSchema_UpdateUnConstrRelationInsertC_eq _ _ H0);
-      [ | eassumption | intros; set_refine_evar; refine pick val (snd r_n'); destruct r_n';
-                        try eauto;
-                        simplify with monad laws; simpl; try finish honing;
-                        unfold H4; instantiate (1 := fun z => ret (snd z, true)); reflexivity].
-    simpl.
-    simpl; unfold UpdateUnConstrRelationInsertC at 1.
-    repeat doOne ltac:(drop_constraints)
-                 drop_constraints_drill ltac:(repeat subst_refine_evar; cbv beta; simpl; try finish honing).
-    doOne ltac:(drop_constraints)
-                 drop_constraints_drill ltac:(repeat subst_refine_evar; cbv beta; simpl; try finish honing).
-    doOne ltac:(drop_constraints)
-                 drop_constraints_drill ltac:(repeat subst_refine_evar; cbv beta; simpl; try finish honing).
-    setoid_rewrite (refine_QueryIn_Where _ _ H0).
-    unfold Tuple_DecomposeRawQueryStructure_inj'; simpl.
-    unfold GetAttribute, GetAttributeRaw at 1; simpl.
-    unfold GetAttribute, GetAttributeRaw at 2; simpl.
-    unfold ilist2_hd; simpl.
-    finish honing.
-    rewrite !refine_if_If.
-    doOne ltac:(drop_constraints)
-                 drop_constraints_drill ltac:(repeat subst_refine_evar; cbv beta; simpl; try finish honing).
-    doOne ltac:(drop_constraints)
-                 drop_constraints_drill ltac:(repeat subst_refine_evar; cbv beta; simpl; try finish honing).
-    doOne ltac:(drop_constraints)
-                 drop_constraints_drill ltac:(repeat subst_refine_evar; cbv beta; simpl; try finish honing).
-        erewrite (DecomposeRawQueryStructureSchema_UpdateUnConstrRelationInsertC_eq _ _ H0);
-      [ | eassumption | intros; set_refine_evar; refine pick val (snd r_n'); destruct r_n';
-                        try eauto;
-                        simplify with monad laws; simpl; try finish honing;
-                        unfold H5; instantiate (1 := fun z => ret (snd z, true)); reflexivity].
-    simpl; unfold UpdateUnConstrRelationInsertC at 1.
-    repeat doOne ltac:(drop_constraints)
-                 drop_constraints_drill ltac:(repeat subst_refine_evar; cbv beta; simpl; try finish honing).
-    repeat doOne ltac:(drop_constraints)
-                        drop_constraints_drill ltac:(repeat subst_refine_evar; cbv beta; simpl; try finish honing).
-    refine pick val _; eauto; finish honing.
-    repeat doOne ltac:(drop_constraints)
-                        drop_constraints_drill ltac:(repeat subst_refine_evar; cbv beta; simpl; try finish honing).
-    refine pick val _; eauto; finish honing.
-  }
-
-  { destruct_ex.
-    doOne ltac:(drop_constraints)
-                 drop_constraints_drill ltac:(repeat subst_refine_evar; cbv beta; simpl; try finish honing).
-    doOne ltac:(drop_constraints)
-                 drop_constraints_drill ltac:(repeat subst_refine_evar; cbv beta; simpl; try finish honing).
-    doOne ltac:(drop_constraints)
-                 drop_constraints_drill ltac:(repeat subst_refine_evar; cbv beta; simpl; try finish honing).
-    doOne ltac:(drop_constraints)
-                 drop_constraints_drill ltac:(repeat subst_refine_evar; cbv beta; simpl; try finish honing).
-    doOne ltac:(drop_constraints)
-                 drop_constraints_drill ltac:(repeat subst_refine_evar; cbv beta; simpl; try finish honing).
-    doOne ltac:(drop_constraints)
-                 drop_constraints_drill ltac:(repeat subst_refine_evar; cbv beta; simpl; try finish honing).
-    doOne ltac:(drop_constraints)
-                 drop_constraints_drill ltac:(repeat subst_refine_evar; cbv beta; simpl; try finish honing).
-    doOne ltac:(drop_constraints)
-                 drop_constraints_drill ltac:(repeat subst_refine_evar; cbv beta; simpl; try finish honing).
-    doOne ltac:(drop_constraints)
-                 drop_constraints_drill ltac:(repeat subst_refine_evar; cbv beta; simpl; try finish honing).
-    rewrite (refine_QueryIn_Where _ _ H0).
-    rewrite (UnConstrQuery_In_Where_Map).
-    rewrite refine_For_Map.
-    doOne ltac:(drop_constraints)
-                 drop_constraints_drill ltac:(repeat subst_refine_evar; cbv beta; simpl; try finish honing).
-    drop_constraints_drill.
-    simpl; finish honing.
-    etransitivity.
-    eapply refine_If_opt_hd_error_map; intros; try eauto.
-    match goal with
-      |- refine (If_Then_Else ?c _ _) _ =>
-      subst_refine_evar; eapply refine_if with (b := c);
-        let H := fresh in
-        intro H; set_refine_evar; try rewrite H; simpl
-    end.
-    rewrite refine_decides_QType_match by eauto.
-    simplify with monad laws.
-    find_if_inside.
-    simpl.
-    doOne ltac:(drop_constraints)
-                 drop_constraints_drill ltac:(repeat subst_refine_evar; cbv beta; simpl; try finish honing).
-    doOne ltac:(drop_constraints)
-                 drop_constraints_drill ltac:(repeat subst_refine_evar; cbv beta; simpl; try finish honing).
-    match type of H2 with
-    | context[ UnConstrQuery_In (qsSchema := ?schem) ?r_n ?R (fun r => Query_Where (@?P r) _)] =>
-      pose proof (@For_UnConstrQuery_In_Where_Prop schem R r_n P a2 _ H2); destruct a2;
-        simpl in *; try discriminate; inversion H7
-    end.
-    simpl in *; injection H4; intros; subst.
-    Local Transparent SumType.SumType_index.
-    Local Transparent SumType.inj_SumType.
-    compute in n; congruence.
-    Local Opaque SumType.SumType_index.
-    Local Opaque SumType.inj_SumType.
-    refine pick val _; eauto.
-    doOne ltac:(drop_constraints)
-                 drop_constraints_drill ltac:(repeat subst_refine_evar; cbv beta; simpl; try finish honing).
-
-    doOne ltac:(drop_constraints)
-                 drop_constraints_drill ltac:(repeat subst_refine_evar; cbv beta; simpl; try finish honing).
-    doOne ltac:(drop_constraints)
-                 drop_constraints_drill ltac:(repeat subst_refine_evar; cbv beta; simpl; try finish honing).
-    doOne ltac:(drop_constraints)
-                 drop_constraints_drill ltac:(repeat subst_refine_evar; cbv beta; simpl; try finish honing).
-    setoid_rewrite refine_If_Then_Bind.
-    rewrite refine_Process_Query_Exact_Match by eassumption.
-    doOne ltac:(drop_constraints)
-                 drop_constraints_drill ltac:(repeat subst_refine_evar; cbv beta; simpl; try finish honing).
-    doOne ltac:(drop_constraints)
-                 drop_constraints_drill ltac:(repeat subst_refine_evar; cbv beta; simpl; try finish honing).
-    rewrite refine_For_List.
-    rewrite (refine_Iterate_Equiv_QueryResultComp _ H0).
-    repeat subst_refine_evar; cbv beta; simpl; try finish honing.
-    doOne ltac:(drop_constraints)
-                 drop_constraints_drill ltac:(repeat subst_refine_evar; cbv beta; simpl; try finish honing).
-    doOne ltac:(drop_constraints)
-                 drop_constraints_drill ltac:(repeat subst_refine_evar; cbv beta; simpl; try finish honing).
-    etransitivity; set_refine_evar.
-    doOne ltac:(drop_constraints)
-                 drop_constraints_drill ltac:(repeat subst_refine_evar; cbv beta; simpl; try finish honing).
-    etransitivity.
-    apply refine_MaxElements'.
-    rewrite (refine_QueryIn_Where _ _ H0).
-    rewrite (UnConstrQuery_In_Where_Map).
-
-    rewrite refine_For_Bind.
-    finish honing.
-
-    rewrite refine_MaxElements_map.
-    finish honing.
-    finish honing.
-    simplify with monad laws.
-
-    doOne ltac:(drop_constraints)
-                 drop_constraints_drill ltac:(repeat subst_refine_evar; cbv beta; simpl; try finish honing).
-    repeat doOne ltac:(drop_constraints)
-                 drop_constraints_drill ltac:(repeat subst_refine_evar; cbv beta; simpl; try finish honing).
-    rewrite refine_filter_Tuple_Decompose_inj'.
-    simplify with monad laws.
-    doOne ltac:(drop_constraints)
-                 drop_constraints_drill ltac:(repeat subst_refine_evar; cbv beta; simpl; try finish honing).
-    doOne ltac:(drop_constraints)
-                 drop_constraints_drill ltac:(repeat subst_refine_evar; cbv beta; simpl; try finish honing).
-    doOne ltac:(drop_constraints)
-                 drop_constraints_drill ltac:(repeat subst_refine_evar; cbv beta; simpl; try finish honing).
-    apply refine_foldComp; intros ? ?; set_refine_evar.
-    rewrite (refine_Iterate_Equiv_QueryResultComp _ H0).
-    Local Opaque Query_For.
-    doOne ltac:(drop_constraints)
-                 drop_constraints_drill ltac:(repeat subst_refine_evar; cbv beta; simpl; try finish honing).
-    doOne ltac:(drop_constraints)
-                 drop_constraints_drill ltac:(repeat subst_refine_evar; cbv beta; simpl; try finish honing).
-    doOne ltac:(drop_constraints)
-                 drop_constraints_drill ltac:(repeat subst_refine_evar; cbv beta; simpl; try finish honing).
-    doOne ltac:(drop_constraints)
-                 drop_constraints_drill ltac:(repeat subst_refine_evar; cbv beta; simpl; try finish honing).
-    doOne ltac:(drop_constraints)
-                 drop_constraints_drill ltac:(repeat subst_refine_evar; cbv beta; simpl; try finish honing).
-    doOne ltac:(drop_constraints)
-                 drop_constraints_drill ltac:(repeat subst_refine_evar; cbv beta; simpl; try finish honing).
-    rewrite (refine_QueryIn_Where _ _ H0).
-    doOne ltac:(drop_constraints)
-                 drop_constraints_drill ltac:(repeat subst_refine_evar; cbv beta; simpl; try finish honing).
-    doOne ltac:(drop_constraints)
-                 drop_constraints_drill ltac:(repeat subst_refine_evar; cbv beta; simpl; try finish honing).
-    rewrite (refine_Iterate_Equiv_QueryResultComp _ H0).
-    doOne ltac:(drop_constraints)
-                 drop_constraints_drill ltac:(repeat subst_refine_evar; cbv beta; simpl; try finish honing).
-    doOne ltac:(drop_constraints)
-                 drop_constraints_drill ltac:(repeat subst_refine_evar; cbv beta; simpl; try finish honing).
-    doOne ltac:(drop_constraints)
-                 drop_constraints_drill ltac:(repeat subst_refine_evar; cbv beta; simpl; try finish honing).
-    etransitivity.
-    doOne ltac:(drop_constraints)
-                 drop_constraints_drill ltac:(repeat subst_refine_evar; cbv beta; simpl; try finish honing).
-    doOne ltac:(drop_constraints)
-                 drop_constraints_drill ltac:(repeat subst_refine_evar; cbv beta; simpl; try finish honing).
-    rewrite (refine_QueryIn_Where _ _ H0).
-    rewrite (UnConstrQuery_In_Where_Map).
-    rewrite refine_For_Bind.
-    finish honing.
-    finish honing.
-    rewrite refine_MaxElements_map.
-    simplify with monad laws.
-    doOne ltac:(drop_constraints)
-                 drop_constraints_drill ltac:(repeat subst_refine_evar; cbv beta; simpl; try finish honing).
-    repeat doOne ltac:(drop_constraints)
-                 drop_constraints_drill ltac:(repeat subst_refine_evar; cbv beta; simpl; try finish honing).
-    rewrite refine_filter_Tuple_Decompose_inj'.
-    simplify with monad laws.
-    doOne ltac:(drop_constraints)
-                 drop_constraints_drill ltac:(repeat subst_refine_evar; cbv beta; simpl; try finish honing).
-    doOne ltac:(drop_constraints)
-                 drop_constraints_drill ltac:(repeat subst_refine_evar; cbv beta; simpl; try finish honing).
-    doOne ltac:(drop_constraints)
-                 drop_constraints_drill ltac:(repeat subst_refine_evar; cbv beta; simpl; try finish honing).
-    apply refine_foldComp; intros ? ?; set_refine_evar.
-    rewrite (refine_Iterate_Equiv_QueryResultComp _ H0).
-    doOne ltac:(drop_constraints)
-                 drop_constraints_drill ltac:(repeat subst_refine_evar; cbv beta; simpl; try finish honing).
-    doOne ltac:(drop_constraints)
-                 drop_constraints_drill ltac:(repeat subst_refine_evar; cbv beta; simpl; try finish honing).
-    doOne ltac:(drop_constraints)
-                 drop_constraints_drill ltac:(repeat subst_refine_evar; cbv beta; simpl; try finish honing).
-    doOne ltac:(drop_constraints)
-                 drop_constraints_drill ltac:(repeat subst_refine_evar; cbv beta; simpl; try finish honing).
-    etransitivity.
-    doOne ltac:(drop_constraints)
-                 drop_constraints_drill ltac:(repeat subst_refine_evar; cbv beta; simpl; try finish honing).
-    apply refine_MaxElements'.
-    rewrite (refine_QueryIn_Where _ _ H0).
-    rewrite (UnConstrQuery_In_Where_Map).
-    rewrite refine_For_Bind.
-    finish honing.
-    finish honing.
-    rewrite refine_MaxElements_map.
-    simplify with monad laws.
-    doOne ltac:(drop_constraints)
-                 drop_constraints_drill ltac:(repeat subst_refine_evar; cbv beta; simpl; try finish honing).
-    repeat doOne ltac:(drop_constraints)
-                 drop_constraints_drill ltac:(repeat subst_refine_evar; cbv beta; simpl; try finish honing).
-    rewrite refine_filter_Tuple_Decompose_inj'.
-    simplify with monad laws.
-    doOne ltac:(drop_constraints)
-                 drop_constraints_drill ltac:(repeat subst_refine_evar; cbv beta; simpl; try finish honing).
-    doOne ltac:(drop_constraints)
-                 drop_constraints_drill ltac:(repeat subst_refine_evar; cbv beta; simpl; try finish honing).
-    doOne ltac:(drop_constraints)
-                 drop_constraints_drill ltac:(repeat subst_refine_evar; cbv beta; simpl; try finish honing).
-    apply refine_foldComp; intros ? ?; set_refine_evar.
-    rewrite (refine_Iterate_Equiv_QueryResultComp _ H0).
-
-    doOne ltac:(drop_constraints)
-                 drop_constraints_drill ltac:(repeat subst_refine_evar; cbv beta; simpl; try finish honing).
-    doOne ltac:(drop_constraints)
-                 drop_constraints_drill ltac:(repeat subst_refine_evar; cbv beta; simpl; try finish honing).
-    doOne ltac:(drop_constraints)
-                 drop_constraints_drill ltac:(repeat subst_refine_evar; cbv beta; simpl; try finish honing).
-    doOne ltac:(drop_constraints)
-                 drop_constraints_drill ltac:(repeat subst_refine_evar; cbv beta; simpl; try finish honing).
-    simpl.
-    finish honing.
-    repeat doOne ltac:(drop_constraints)
-                 drop_constraints_drill ltac:(repeat subst_refine_evar; cbv beta; simpl; try finish honing).
-    refine pick val _; eauto; finish honing.
-    repeat doOne ltac:(drop_constraints)
-                 drop_constraints_drill ltac:(repeat subst_refine_evar; cbv beta; simpl; try finish honing).
-    refine pick val _; eauto; finish honing.
-  }
-  simpl.
-  pose {| prim_fst := [(EqualityIndex, @Fin.F1 3)];
-          prim_snd := {|
-          prim_fst := [(EqualityIndex, @Fin.F1 3)];
-          prim_snd := {|
-          prim_fst := [(FindStringPrefixIndex, @Fin.F1 3)];
-          prim_snd := {|
-          prim_fst := [(EqualityIndex, @Fin.F1 3)];
-          prim_snd := () |} |} |} |}.
-
-  Time let p' := eval unfold p in p in
-           make_simple_indexes p'
-                               ltac:(CombineCase6 BuildEarlyFindStringPrefixIndex ltac:(LastCombineCase6 BuildEarlyEqualityIndex))
-                                      ltac:(CombineCase5 BuildLastStringFindPrefixIndex ltac:(LastCombineCase5 BuildLastEqualityIndex)).
-
-    { (* Constructor *)
-      Unset Ltac Debug.
-      initializer.
-    }
-    Focus 2.
-    {
-      doOne implement_insert''
-            ltac:(master_implement_drill
-          ltac:(CombineCase5 StringPrefixIndexUse EqIndexUse)
-          ltac:(CombineCase10 createEarlyStringPrefixTerm createEarlyEqualityTerm)
-          ltac:(CombineCase7 createLastStringPrefixTerm createLastEqualityTerm);
-      set_evars) ltac:(finish honing).
-
-    { (* Add Data *)
-    doOne implement_insert''
-          ltac:(master_implement_drill
-          ltac:(CombineCase5 StringPrefixIndexUse EqIndexUse)
-          ltac:(CombineCase10 createEarlyStringPrefixTerm createEarlyEqualityTerm)
-          ltac:(CombineCase7 createLastStringPrefixTerm createLastEqualityTerm);
-      set_evars) ltac:(finish honing).
-    doOne implement_insert''
-          ltac:(master_implement_drill
-          ltac:(CombineCase5 StringPrefixIndexUse EqIndexUse)
-          ltac:(CombineCase10 createEarlyStringPrefixTerm createEarlyEqualityTerm)
-          ltac:(CombineCase7 createLastStringPrefixTerm createLastEqualityTerm);
-      set_evars) ltac:(finish honing).
-    doOne implement_insert''
-          ltac:(master_implement_drill
-          ltac:(CombineCase5 StringPrefixIndexUse EqIndexUse)
-          ltac:(CombineCase10 createEarlyStringPrefixTerm createEarlyEqualityTerm)
-          ltac:(CombineCase7 createLastStringPrefixTerm createLastEqualityTerm);
-      set_evars) ltac:(finish honing).
-    doOne implement_insert''
+    Time doOne implement_insert'''
           ltac:(master_implement_drill
           ltac:(CombineCase5 StringPrefixIndexUse EqIndexUse)
           ltac:(CombineCase10 createEarlyStringPrefixTerm createEarlyEqualityTerm)
           ltac:(CombineCase7 createLastStringPrefixTerm createLastEqualityTerm);
                 set_evars) ltac:(finish honing).
-    refine pick val 0.
-    doOne implement_insert''
+    Time doOne implement_insert'''
           ltac:(master_implement_drill
           ltac:(CombineCase5 StringPrefixIndexUse EqIndexUse)
           ltac:(CombineCase10 createEarlyStringPrefixTerm createEarlyEqualityTerm)
           ltac:(CombineCase7 createLastStringPrefixTerm createLastEqualityTerm);
                 set_evars) ltac:(finish honing).
-    admit.
-    doOne implement_insert''
+    Time doOne implement_insert'''
           ltac:(master_implement_drill
           ltac:(CombineCase5 StringPrefixIndexUse EqIndexUse)
           ltac:(CombineCase10 createEarlyStringPrefixTerm createEarlyEqualityTerm)
           ltac:(CombineCase7 createLastStringPrefixTerm createLastEqualityTerm);
                 set_evars) ltac:(finish honing).
-    doOne implement_insert''
-          ltac:(master_implement_drill
-          ltac:(CombineCase5 StringPrefixIndexUse EqIndexUse)
-          ltac:(CombineCase10 createEarlyStringPrefixTerm createEarlyEqualityTerm)
-          ltac:(CombineCase7 createLastStringPrefixTerm createLastEqualityTerm);
-      set_evars) ltac:(finish honing).
-
-    doOne implement_insert''
-          ltac:(master_implement_drill
-          ltac:(CombineCase5 StringPrefixIndexUse EqIndexUse)
-          ltac:(CombineCase10 createEarlyStringPrefixTerm createEarlyEqualityTerm)
-          ltac:(CombineCase7 createLastStringPrefixTerm createLastEqualityTerm);
-      set_evars) ltac:(finish honing).
-    doOne implement_insert''
-          ltac:(master_implement_drill
-          ltac:(CombineCase5 StringPrefixIndexUse EqIndexUse)
-          ltac:(CombineCase10 createEarlyStringPrefixTerm createEarlyEqualityTerm)
-          ltac:(CombineCase7 createLastStringPrefixTerm createLastEqualityTerm);
-      set_evars) ltac:(finish honing).
-    doOne implement_insert''
+    Time doOne implement_insert'''
           ltac:(master_implement_drill
           ltac:(CombineCase5 StringPrefixIndexUse EqIndexUse)
           ltac:(CombineCase10 createEarlyStringPrefixTerm createEarlyEqualityTerm)
           ltac:(CombineCase7 createLastStringPrefixTerm createLastEqualityTerm);
                 set_evars) ltac:(finish honing).
-    doOne implement_insert''
-          ltac:(master_implement_drill
-          ltac:(CombineCase5 StringPrefixIndexUse EqIndexUse)
-          ltac:(CombineCase10 createEarlyStringPrefixTerm createEarlyEqualityTerm)
-          ltac:(CombineCase7 createLastStringPrefixTerm createLastEqualityTerm);
-      set_evars) ltac:(finish honing).
-    doAny implement_insert''
-          ltac:(master_implement_drill
-          ltac:(CombineCase5 StringPrefixIndexUse EqIndexUse)
-          ltac:(CombineCase10 createEarlyStringPrefixTerm createEarlyEqualityTerm)
-          ltac:(CombineCase7 createLastStringPrefixTerm createLastEqualityTerm);
-      set_evars) ltac:(finish honing).
-    doOne implement_insert''
-          ltac:(master_implement_drill
-          ltac:(CombineCase5 StringPrefixIndexUse EqIndexUse)
-          ltac:(CombineCase10 createEarlyStringPrefixTerm createEarlyEqualityTerm)
-          ltac:(CombineCase7 createLastStringPrefixTerm createLastEqualityTerm);
-      set_evars) ltac:(finish honing).
-    doOne implement_insert''
-          ltac:(master_implement_drill
-          ltac:(CombineCase5 StringPrefixIndexUse EqIndexUse)
-          ltac:(CombineCase10 createEarlyStringPrefixTerm createEarlyEqualityTerm)
-          ltac:(CombineCase7 createLastStringPrefixTerm createLastEqualityTerm);
-      set_evars) ltac:(finish honing).
-    doOne implement_insert''
-          ltac:(master_implement_drill
-          ltac:(CombineCase5 StringPrefixIndexUse EqIndexUse)
-          ltac:(CombineCase10 createEarlyStringPrefixTerm createEarlyEqualityTerm)
-          ltac:(CombineCase7 createLastStringPrefixTerm createLastEqualityTerm);
-      set_evars) ltac:(finish honing).
-    doAny implement_insert''
-          ltac:(master_implement_drill
-          ltac:(CombineCase5 StringPrefixIndexUse EqIndexUse)
-          ltac:(CombineCase10 createEarlyStringPrefixTerm createEarlyEqualityTerm)
-          ltac:(CombineCase7 createLastStringPrefixTerm createLastEqualityTerm);
-      set_evars) ltac:(finish honing).
-    doOne implement_insert''
-          ltac:(master_implement_drill
-          ltac:(CombineCase5 StringPrefixIndexUse EqIndexUse)
-          ltac:(CombineCase10 createEarlyStringPrefixTerm createEarlyEqualityTerm)
-          ltac:(CombineCase7 createLastStringPrefixTerm createLastEqualityTerm);
-      set_evars) ltac:(finish honing).
-    doAny implement_insert''
-          ltac:(master_implement_drill
-          ltac:(CombineCase5 StringPrefixIndexUse EqIndexUse)
-          ltac:(CombineCase10 createEarlyStringPrefixTerm createEarlyEqualityTerm)
-          ltac:(CombineCase7 createLastStringPrefixTerm createLastEqualityTerm);
-      set_evars) ltac:(finish honing).
-  }
-  doOne implement_insert''
-          ltac:(master_implement_drill
-          ltac:(CombineCase5 StringPrefixIndexUse EqIndexUse)
-          ltac:(CombineCase10 createEarlyStringPrefixTerm createEarlyEqualityTerm)
-          ltac:(CombineCase7 createLastStringPrefixTerm createLastEqualityTerm);
-      set_evars) ltac:(finish honing).
-    doOne implement_insert''
-          ltac:(master_implement_drill
-          ltac:(CombineCase5 StringPrefixIndexUse EqIndexUse)
-          ltac:(CombineCase10 createEarlyStringPrefixTerm createEarlyEqualityTerm)
-          ltac:(CombineCase7 createLastStringPrefixTerm createLastEqualityTerm);
-      set_evars) ltac:(finish honing).
-    doOne implement_insert''
-          ltac:(master_implement_drill
-          ltac:(CombineCase5 StringPrefixIndexUse EqIndexUse)
-          ltac:(CombineCase10 createEarlyStringPrefixTerm createEarlyEqualityTerm)
-          ltac:(CombineCase7 createLastStringPrefixTerm createLastEqualityTerm);
-      set_evars) ltac:(finish honing).
-    doOne implement_insert''
-          ltac:(master_implement_drill
-          ltac:(CombineCase5 StringPrefixIndexUse EqIndexUse)
-          ltac:(CombineCase10 createEarlyStringPrefixTerm createEarlyEqualityTerm)
-          ltac:(CombineCase7 createLastStringPrefixTerm createLastEqualityTerm);
-      set_evars) ltac:(finish honing).
-    doOne implement_insert''
-          ltac:(master_implement_drill
-          ltac:(CombineCase5 StringPrefixIndexUse EqIndexUse)
-          ltac:(CombineCase10 createEarlyStringPrefixTerm createEarlyEqualityTerm)
-          ltac:(CombineCase7 createLastStringPrefixTerm createLastEqualityTerm);
-      set_evars) ltac:(finish honing).
-    doOne implement_insert''
-          ltac:(master_implement_drill
-          ltac:(CombineCase5 StringPrefixIndexUse EqIndexUse)
-          ltac:(CombineCase10 createEarlyStringPrefixTerm createEarlyEqualityTerm)
-          ltac:(CombineCase7 createLastStringPrefixTerm createLastEqualityTerm);
-      set_evars) ltac:(finish honing).
-    doOne implement_insert''
-          ltac:(master_implement_drill
-          ltac:(CombineCase5 StringPrefixIndexUse EqIndexUse)
-          ltac:(CombineCase10 createEarlyStringPrefixTerm createEarlyEqualityTerm)
-          ltac:(CombineCase7 createLastStringPrefixTerm createLastEqualityTerm);
-      set_evars) ltac:(finish honing).
-    eapply refineFueledFix.
-    finish honing.
-    intros.
-    doOne implement_insert''
+    Time doOne implement_insert'''
           ltac:(master_implement_drill
           ltac:(CombineCase5 StringPrefixIndexUse EqIndexUse)
           ltac:(CombineCase10 createEarlyStringPrefixTerm createEarlyEqualityTerm)
           ltac:(CombineCase7 createLastStringPrefixTerm createLastEqualityTerm);
                 set_evars) ltac:(finish honing).
-    implement_insert''.
-    doOne implement_insert''
+    Time doOne implement_insert'''
           ltac:(master_implement_drill
           ltac:(CombineCase5 StringPrefixIndexUse EqIndexUse)
           ltac:(CombineCase10 createEarlyStringPrefixTerm createEarlyEqualityTerm)
           ltac:(CombineCase7 createLastStringPrefixTerm createLastEqualityTerm);
                 set_evars) ltac:(finish honing).
-    doOne implement_insert''
+    Time doOne implement_insert'''
           ltac:(master_implement_drill
           ltac:(CombineCase5 StringPrefixIndexUse EqIndexUse)
           ltac:(CombineCase10 createEarlyStringPrefixTerm createEarlyEqualityTerm)
           ltac:(CombineCase7 createLastStringPrefixTerm createLastEqualityTerm);
                 set_evars) ltac:(finish honing).
-    doAny implement_insert''
+    Time doOne implement_insert'''
           ltac:(master_implement_drill
           ltac:(CombineCase5 StringPrefixIndexUse EqIndexUse)
           ltac:(CombineCase10 createEarlyStringPrefixTerm createEarlyEqualityTerm)
           ltac:(CombineCase7 createLastStringPrefixTerm createLastEqualityTerm);
                 set_evars) ltac:(finish honing).
-    doOne implement_insert''
+    Time doOne implement_insert'''
           ltac:(master_implement_drill
           ltac:(CombineCase5 StringPrefixIndexUse EqIndexUse)
           ltac:(CombineCase10 createEarlyStringPrefixTerm createEarlyEqualityTerm)
           ltac:(CombineCase7 createLastStringPrefixTerm createLastEqualityTerm);
                 set_evars) ltac:(finish honing).
-    doOne implement_insert''
+    Time doOne implement_insert'''
           ltac:(master_implement_drill
           ltac:(CombineCase5 StringPrefixIndexUse EqIndexUse)
           ltac:(CombineCase10 createEarlyStringPrefixTerm createEarlyEqualityTerm)
           ltac:(CombineCase7 createLastStringPrefixTerm createLastEqualityTerm);
                 set_evars) ltac:(finish honing).
-    doOne implement_insert''
+    Time doOne implement_insert'''
           ltac:(master_implement_drill
           ltac:(CombineCase5 StringPrefixIndexUse EqIndexUse)
           ltac:(CombineCase10 createEarlyStringPrefixTerm createEarlyEqualityTerm)
           ltac:(CombineCase7 createLastStringPrefixTerm createLastEqualityTerm);
                 set_evars) ltac:(finish honing).
-    doOne implement_insert''
+    Time doOne implement_insert'''
           ltac:(master_implement_drill
           ltac:(CombineCase5 StringPrefixIndexUse EqIndexUse)
           ltac:(CombineCase10 createEarlyStringPrefixTerm createEarlyEqualityTerm)
           ltac:(CombineCase7 createLastStringPrefixTerm createLastEqualityTerm);
                 set_evars) ltac:(finish honing).
-    doOne implement_insert''
+    Time doOne implement_insert'''
+          ltac:(master_implement_drill
+          ltac:(CombineCase5 StringPrefixIndexUse EqIndexUse)
+          ltac:(CombineCase10 createEarlyStringPrefixTerm createEarlyEqualityTerm)
+          ltac:(CombineCase7 createLastStringPrefixTerm createLastEqualityTerm);
+                set_evars) ltac:(finish honing).
+    Time doOne implement_insert'''
+          ltac:(master_implement_drill
+          ltac:(CombineCase5 StringPrefixIndexUse EqIndexUse)
+          ltac:(CombineCase10 createEarlyStringPrefixTerm createEarlyEqualityTerm)
+          ltac:(CombineCase7 createLastStringPrefixTerm createLastEqualityTerm);
+                set_evars) ltac:(finish honing).
+   Time doOne implement_insert'''
+          ltac:(master_implement_drill
+          ltac:(CombineCase5 StringPrefixIndexUse EqIndexUse)
+          ltac:(CombineCase10 createEarlyStringPrefixTerm createEarlyEqualityTerm)
+          ltac:(CombineCase7 createLastStringPrefixTerm createLastEqualityTerm);
+                set_evars) ltac:(finish honing).
+    Time doOne implement_insert'''
+          ltac:(master_implement_drill
+          ltac:(CombineCase5 StringPrefixIndexUse EqIndexUse)
+          ltac:(CombineCase10 createEarlyStringPrefixTerm createEarlyEqualityTerm)
+          ltac:(CombineCase7 createLastStringPrefixTerm createLastEqualityTerm);
+                set_evars) ltac:(finish honing).
+    Time doOne implement_insert'''
+          ltac:(master_implement_drill
+          ltac:(CombineCase5 StringPrefixIndexUse EqIndexUse)
+          ltac:(CombineCase10 createEarlyStringPrefixTerm createEarlyEqualityTerm)
+          ltac:(CombineCase7 createLastStringPrefixTerm createLastEqualityTerm);
+                set_evars) ltac:(finish honing).
+    Time doOne implement_insert'''
+          ltac:(master_implement_drill
+          ltac:(CombineCase5 StringPrefixIndexUse EqIndexUse)
+          ltac:(CombineCase10 createEarlyStringPrefixTerm createEarlyEqualityTerm)
+          ltac:(CombineCase7 createLastStringPrefixTerm createLastEqualityTerm);
+                set_evars) ltac:(finish honing).
+    Time doOne implement_insert'''
+          ltac:(master_implement_drill
+          ltac:(CombineCase5 StringPrefixIndexUse EqIndexUse)
+          ltac:(CombineCase10 createEarlyStringPrefixTerm createEarlyEqualityTerm)
+          ltac:(CombineCase7 createLastStringPrefixTerm createLastEqualityTerm);
+                set_evars) ltac:(finish honing).
+    Time doOne implement_insert'''
+          ltac:(master_implement_drill
+          ltac:(CombineCase5 StringPrefixIndexUse EqIndexUse)
+          ltac:(CombineCase10 createEarlyStringPrefixTerm createEarlyEqualityTerm)
+          ltac:(CombineCase7 createLastStringPrefixTerm createLastEqualityTerm);
+                set_evars) ltac:(finish honing).
+    Time doOne implement_insert'''
           ltac:(master_implement_drill
           ltac:(CombineCase5 StringPrefixIndexUse EqIndexUse)
           ltac:(CombineCase10 createEarlyStringPrefixTerm createEarlyEqualityTerm)
           ltac:(CombineCase7 createLastStringPrefixTerm createLastEqualityTerm);
                 set_evars) ltac:(finish honing).
 
-        doOne implement_insert''
-          ltac:(master_implement_drill
-          ltac:(CombineCase5 StringPrefixIndexUse EqIndexUse)
-          ltac:(CombineCase10 createEarlyStringPrefixTerm createEarlyEqualityTerm)
-          ltac:(CombineCase7 createLastStringPrefixTerm createLastEqualityTerm);
-                set_evars) ltac:(finish honing).
-    doOne implement_insert''
-          ltac:(master_implement_drill
-          ltac:(CombineCase5 StringPrefixIndexUse EqIndexUse)
-          ltac:(CombineCase10 createEarlyStringPrefixTerm createEarlyEqualityTerm)
-          ltac:(CombineCase7 createLastStringPrefixTerm createLastEqualityTerm);
-                set_evars) ltac:(finish honing).
-    doOne implement_insert''
-          ltac:(master_implement_drill
-          ltac:(CombineCase5 StringPrefixIndexUse EqIndexUse)
-          ltac:(CombineCase10 createEarlyStringPrefixTerm createEarlyEqualityTerm)
-          ltac:(CombineCase7 createLastStringPrefixTerm createLastEqualityTerm);
-                set_evars) ltac:(finish honing).
-    doOne implement_insert''
-          ltac:(master_implement_drill
-          ltac:(CombineCase5 StringPrefixIndexUse EqIndexUse)
-          ltac:(CombineCase10 createEarlyStringPrefixTerm createEarlyEqualityTerm)
-          ltac:(CombineCase7 createLastStringPrefixTerm createLastEqualityTerm);
-                set_evars) ltac:(finish honing).
-    doOne implement_insert''
-          ltac:(master_implement_drill
-          ltac:(CombineCase5 StringPrefixIndexUse EqIndexUse)
-          ltac:(CombineCase10 createEarlyStringPrefixTerm createEarlyEqualityTerm)
-          ltac:(CombineCase7 createLastStringPrefixTerm createLastEqualityTerm);
-                set_evars) ltac:(finish honing).
-    rewrite H2.
 
-    doOne implement_insert''
-          ltac:(master_implement_drill
-          ltac:(CombineCase5 StringPrefixIndexUse EqIndexUse)
-          ltac:(CombineCase10 createEarlyStringPrefixTerm createEarlyEqualityTerm)
-          ltac:(CombineCase7 createLastStringPrefixTerm createLastEqualityTerm);
-                set_evars) ltac:(finish honing).
-    doOne implement_insert''
-          ltac:(master_implement_drill
-          ltac:(CombineCase5 StringPrefixIndexUse EqIndexUse)
-          ltac:(CombineCase10 createEarlyStringPrefixTerm createEarlyEqualityTerm)
-          ltac:(CombineCase7 createLastStringPrefixTerm createLastEqualityTerm);
-                set_evars) ltac:(finish honing).
-    doOne implement_insert''
-          ltac:(master_implement_drill
-          ltac:(CombineCase5 StringPrefixIndexUse EqIndexUse)
-          ltac:(CombineCase10 createEarlyStringPrefixTerm createEarlyEqualityTerm)
-          ltac:(CombineCase7 createLastStringPrefixTerm createLastEqualityTerm);
-                set_evars) ltac:(finish honing).
-    doOne implement_insert''
-          ltac:(master_implement_drill
-          ltac:(CombineCase5 StringPrefixIndexUse EqIndexUse)
-          ltac:(CombineCase10 createEarlyStringPrefixTerm createEarlyEqualityTerm)
-          ltac:(CombineCase7 createLastStringPrefixTerm createLastEqualityTerm);
-                set_evars) ltac:(finish honing).
-    doOne implement_insert''
+    Time doOne implement_insert'''
           ltac:(master_implement_drill
           ltac:(CombineCase5 StringPrefixIndexUse EqIndexUse)
           ltac:(CombineCase10 createEarlyStringPrefixTerm createEarlyEqualityTerm)
           ltac:(CombineCase7 createLastStringPrefixTerm createLastEqualityTerm);
                 set_evars) ltac:(finish honing).
 
-        doOne implement_insert''
+    simplify_Query_Where'.
+
+    Time doOne implement_insert'''
           ltac:(master_implement_drill
           ltac:(CombineCase5 StringPrefixIndexUse EqIndexUse)
           ltac:(CombineCase10 createEarlyStringPrefixTerm createEarlyEqualityTerm)
           ltac:(CombineCase7 createLastStringPrefixTerm createLastEqualityTerm);
                 set_evars) ltac:(finish honing).
-    doOne implement_insert''
+    simplify_Query_Where'.
+    subst_refine_evar; eapply refine_under_bind_both;
+    try set_refine_evar; intros.
+    repeat  doOne implement_insert'''
           ltac:(master_implement_drill
           ltac:(CombineCase5 StringPrefixIndexUse EqIndexUse)
           ltac:(CombineCase10 createEarlyStringPrefixTerm createEarlyEqualityTerm)
           ltac:(CombineCase7 createLastStringPrefixTerm createLastEqualityTerm);
                 set_evars) ltac:(finish honing).
-    doOne implement_insert''
+    simplify_Query_Where'.
+    subst_refine_evar; eapply refine_under_bind_both;
+    try set_refine_evar; intros.
+    repeat  doOne implement_insert'''
           ltac:(master_implement_drill
           ltac:(CombineCase5 StringPrefixIndexUse EqIndexUse)
           ltac:(CombineCase10 createEarlyStringPrefixTerm createEarlyEqualityTerm)
           ltac:(CombineCase7 createLastStringPrefixTerm createLastEqualityTerm);
                 set_evars) ltac:(finish honing).
-    Focused_refine_TopMost_Query.
+    simplify_Query_Where'.
+    subst_refine_evar; eapply refine_under_bind_both;
+    try set_refine_evar; intros.
+    repeat  doOne implement_insert'''
+          ltac:(master_implement_drill
+          ltac:(CombineCase5 StringPrefixIndexUse EqIndexUse)
+          ltac:(CombineCase10 createEarlyStringPrefixTerm createEarlyEqualityTerm)
+          ltac:(CombineCase7 createLastStringPrefixTerm createLastEqualityTerm);
+                set_evars) ltac:(finish honing).
+    simplify_Query_Where'.
+    subst_refine_evar; eapply refine_under_bind_both;
+    try set_refine_evar; intros.
+    repeat  doOne implement_insert'''
+          ltac:(master_implement_drill
+          ltac:(CombineCase5 StringPrefixIndexUse EqIndexUse)
+          ltac:(CombineCase10 createEarlyStringPrefixTerm createEarlyEqualityTerm)
+          ltac:(CombineCase7 createLastStringPrefixTerm createLastEqualityTerm);
+                set_evars) ltac:(finish honing).
+    simplify_Query_Where'.
+    subst_refine_evar; eapply refine_under_bind_both;
+    try set_refine_evar; intros.
+    repeat  doOne implement_insert'''
+          ltac:(master_implement_drill
+          ltac:(CombineCase5 StringPrefixIndexUse EqIndexUse)
+          ltac:(CombineCase10 createEarlyStringPrefixTerm createEarlyEqualityTerm)
+          ltac:(CombineCase7 createLastStringPrefixTerm createLastEqualityTerm);
+                set_evars) ltac:(finish honing).
+    rewrite refine_unit_bind'.
+
+
+    repeat doOne implement_insert'''
+          ltac:(master_implement_drill
+          ltac:(CombineCase5 StringPrefixIndexUse EqIndexUse)
+          ltac:(CombineCase10 createEarlyStringPrefixTerm createEarlyEqualityTerm)
+          ltac:(CombineCase7 createLastStringPrefixTerm createLastEqualityTerm);
+                set_evars) ltac:(finish honing).
+    simplify_Query_Where'.
+    subst_refine_evar; eapply refine_under_bind_both;
+    try set_refine_evar; intros.
+    repeat  doOne implement_insert'''
+          ltac:(master_implement_drill
+          ltac:(CombineCase5 StringPrefixIndexUse EqIndexUse)
+          ltac:(CombineCase10 createEarlyStringPrefixTerm createEarlyEqualityTerm)
+          ltac:(CombineCase7 createLastStringPrefixTerm createLastEqualityTerm);
+                set_evars) ltac:(finish honing).
+    rewrite refine_unit_bind'.
+    repeat doOne implement_insert'''
+           ltac:(master_implement_drill
+          ltac:(CombineCase5 StringPrefixIndexUse EqIndexUse)
+          ltac:(CombineCase10 createEarlyStringPrefixTerm createEarlyEqualityTerm)
+          ltac:(CombineCase7 createLastStringPrefixTerm createLastEqualityTerm);
+                set_evars) ltac:(finish honing).
+    simplify_Query_Where'.
+    subst_refine_evar; eapply refine_under_bind_both;
+    try set_refine_evar; intros.
+    repeat  doOne implement_insert'''
+          ltac:(master_implement_drill
+          ltac:(CombineCase5 StringPrefixIndexUse EqIndexUse)
+          ltac:(CombineCase10 createEarlyStringPrefixTerm createEarlyEqualityTerm)
+          ltac:(CombineCase7 createLastStringPrefixTerm createLastEqualityTerm);
+                set_evars) ltac:(finish honing).
+    rewrite refine_unit_bind'.
+    repeat doOne implement_insert'''
+           ltac:(master_implement_drill
+          ltac:(CombineCase5 StringPrefixIndexUse EqIndexUse)
+          ltac:(CombineCase10 createEarlyStringPrefixTerm createEarlyEqualityTerm)
+          ltac:(CombineCase7 createLastStringPrefixTerm createLastEqualityTerm);
+                set_evars) ltac:(finish honing).
+    Time doOne implement_insert'''
+          ltac:(master_implement_drill
+          ltac:(CombineCase5 StringPrefixIndexUse EqIndexUse)
+          ltac:(CombineCase10 createEarlyStringPrefixTerm createEarlyEqualityTerm)
+          ltac:(CombineCase7 createLastStringPrefixTerm createLastEqualityTerm);
+                set_evars) ltac:(finish honing).
     set_refine_evar.
-    etransitivity.
-    match goal with
-      | [H : @DelegateToBag_AbsR ?qs_schema ?indexes ?r_o ?r_n
-     |- refine (UnConstrQuery_In (ResultT := ?resultT) ?r_o ?idx ?f) _ ] =>
-    etransitivity;
-      [ let H' := eval simpl in (refine_Filtered_Query_In_Enumerate H (idx := idx) f) in
-            apply H'
-      | apply refine_under_bind; intros]
-    end.
-    match goal with
-    | [H : @DelegateToBag_AbsR ?qs_schema ?indexes ?r_o ?r_n
-       |- refine (List_Query_In ?b (fun b : ?QueryT => Where (@?P b) (@?resultComp b))) _ ] =>
-      etransitivity;
-        [ let H' := eval simpl in (@refine_List_Query_In_Where QueryT _ b P resultComp) in
-              pose proof H' | ]
-    end.
-    simpl in H10.
-    Check (H10 _). P_dec : DecideableEnsemble
-                    (fun
-                       tup : ilist2
-                               [{| NumAttr := 5; AttrList := [DomainName; timeT; RRecordClass; RRecordType; RDataType] |}]%NamedSchema =>
-                     List.In (GetAttributeRaw (ilist2_hd tup) Fin.F1)
-                       (map (fun r : NS_Record => GetAttributeRaw r (Fin.FS (Fin.FS (Fin.FS (Fin.FS Fin.F1))))) a5))
-
-
-    etransitivity.
-    let H' := eval simpl in (refine_Filtered_Query_In_Enumerate H (idx := idx) f) in
-        apply H'
-      | apply refine_under_bind; intros; implement_In_opt' ]
-
-    implement_In_opt.
-    repeat progress distribute_filters_to_joins.
-    (* Step 3: Convert filter function on topmost [Join_Filtered_Comp_Lists] to an
-               equivalent search term matching function.  *)
-    implement_filters_with_find k k_dep
-  |
-  ]; pose_string_hyps; pose_heading_hyps.
-    doOne implement_insert''
+    Time doOne implement_insert'''
           ltac:(master_implement_drill
           ltac:(CombineCase5 StringPrefixIndexUse EqIndexUse)
           ltac:(CombineCase10 createEarlyStringPrefixTerm createEarlyEqualityTerm)
           ltac:(CombineCase7 createLastStringPrefixTerm createLastEqualityTerm);
                 set_evars) ltac:(finish honing).
-    doOne implement_insert''
+    Time doOne implement_insert'''
           ltac:(master_implement_drill
           ltac:(CombineCase5 StringPrefixIndexUse EqIndexUse)
           ltac:(CombineCase10 createEarlyStringPrefixTerm createEarlyEqualityTerm)
           ltac:(CombineCase7 createLastStringPrefixTerm createLastEqualityTerm);
                 set_evars) ltac:(finish honing).
-
-        doOne implement_insert''
+    Time doOne implement_insert'''
           ltac:(master_implement_drill
           ltac:(CombineCase5 StringPrefixIndexUse EqIndexUse)
           ltac:(CombineCase10 createEarlyStringPrefixTerm createEarlyEqualityTerm)
           ltac:(CombineCase7 createLastStringPrefixTerm createLastEqualityTerm);
                 set_evars) ltac:(finish honing).
-    doOne implement_insert''
+    rewrite refine_MaxPrefix.
+    Time doOne implement_insert'''
           ltac:(master_implement_drill
           ltac:(CombineCase5 StringPrefixIndexUse EqIndexUse)
           ltac:(CombineCase10 createEarlyStringPrefixTerm createEarlyEqualityTerm)
           ltac:(CombineCase7 createLastStringPrefixTerm createLastEqualityTerm);
                 set_evars) ltac:(finish honing).
-    doOne implement_insert''
+    repeat doOne implement_insert'''
           ltac:(master_implement_drill
           ltac:(CombineCase5 StringPrefixIndexUse EqIndexUse)
           ltac:(CombineCase10 createEarlyStringPrefixTerm createEarlyEqualityTerm)
           ltac:(CombineCase7 createLastStringPrefixTerm createLastEqualityTerm);
                 set_evars) ltac:(finish honing).
-    doOne implement_insert''
+    Time doOne implement_insert'''
           ltac:(master_implement_drill
           ltac:(CombineCase5 StringPrefixIndexUse EqIndexUse)
           ltac:(CombineCase10 createEarlyStringPrefixTerm createEarlyEqualityTerm)
           ltac:(CombineCase7 createLastStringPrefixTerm createLastEqualityTerm);
                 set_evars) ltac:(finish honing).
-    doOne implement_insert''
+    Time doOne implement_insert'''
           ltac:(master_implement_drill
           ltac:(CombineCase5 StringPrefixIndexUse EqIndexUse)
           ltac:(CombineCase10 createEarlyStringPrefixTerm createEarlyEqualityTerm)
           ltac:(CombineCase7 createLastStringPrefixTerm createLastEqualityTerm);
                 set_evars) ltac:(finish honing).
-
-        doOne implement_insert''
+    Time doOne implement_insert'''
           ltac:(master_implement_drill
           ltac:(CombineCase5 StringPrefixIndexUse EqIndexUse)
           ltac:(CombineCase10 createEarlyStringPrefixTerm createEarlyEqualityTerm)
           ltac:(CombineCase7 createLastStringPrefixTerm createLastEqualityTerm);
                 set_evars) ltac:(finish honing).
-    doOne implement_insert''
+    apply refine_foldComp; intros ? ?; set_refine_evar.
+    repeat doOne implement_insert'''
           ltac:(master_implement_drill
           ltac:(CombineCase5 StringPrefixIndexUse EqIndexUse)
           ltac:(CombineCase10 createEarlyStringPrefixTerm createEarlyEqualityTerm)
           ltac:(CombineCase7 createLastStringPrefixTerm createLastEqualityTerm);
                 set_evars) ltac:(finish honing).
-    doOne implement_insert''
+    repeat doOne implement_insert'''
           ltac:(master_implement_drill
           ltac:(CombineCase5 StringPrefixIndexUse EqIndexUse)
           ltac:(CombineCase10 createEarlyStringPrefixTerm createEarlyEqualityTerm)
           ltac:(CombineCase7 createLastStringPrefixTerm createLastEqualityTerm);
                 set_evars) ltac:(finish honing).
-    doOne implement_insert''
+    rewrite refine_MaxPrefix.
+    Time doOne implement_insert'''
           ltac:(master_implement_drill
           ltac:(CombineCase5 StringPrefixIndexUse EqIndexUse)
           ltac:(CombineCase10 createEarlyStringPrefixTerm createEarlyEqualityTerm)
           ltac:(CombineCase7 createLastStringPrefixTerm createLastEqualityTerm);
                 set_evars) ltac:(finish honing).
-    doOne implement_insert''
+    Time doOne implement_insert'''
           ltac:(master_implement_drill
           ltac:(CombineCase5 StringPrefixIndexUse EqIndexUse)
           ltac:(CombineCase10 createEarlyStringPrefixTerm createEarlyEqualityTerm)
           ltac:(CombineCase7 createLastStringPrefixTerm createLastEqualityTerm);
                 set_evars) ltac:(finish honing).
-
-
-
-  { (* Add Data. *)
-  plan EqIndexUse createEarlyEqualityTerm createLastEqualityTerm
-       EqIndexUse_dep createEarlyEqualityTerm_dep createLastEqualityTerm_dep.
-
+    Time doOne implement_insert'''
+          ltac:(master_implement_drill
+          ltac:(CombineCase5 StringPrefixIndexUse EqIndexUse)
+          ltac:(CombineCase10 createEarlyStringPrefixTerm createEarlyEqualityTerm)
+          ltac:(CombineCase7 createLastStringPrefixTerm createLastEqualityTerm);
+                set_evars) ltac:(finish honing).
+    Time doOne implement_insert'''
+          ltac:(master_implement_drill
+          ltac:(CombineCase5 StringPrefixIndexUse EqIndexUse)
+          ltac:(CombineCase10 createEarlyStringPrefixTerm createEarlyEqualityTerm)
+          ltac:(CombineCase7 createLastStringPrefixTerm createLastEqualityTerm);
+                set_evars) ltac:(finish honing).
+    Time doOne implement_insert'''
+          ltac:(master_implement_drill
+          ltac:(CombineCase5 StringPrefixIndexUse EqIndexUse)
+          ltac:(CombineCase10 createEarlyStringPrefixTerm createEarlyEqualityTerm)
+          ltac:(CombineCase7 createLastStringPrefixTerm createLastEqualityTerm);
+                set_evars) ltac:(finish honing).
+    Time doOne implement_insert'''
+          ltac:(master_implement_drill
+          ltac:(CombineCase5 StringPrefixIndexUse EqIndexUse)
+          ltac:(CombineCase10 createEarlyStringPrefixTerm createEarlyEqualityTerm)
+          ltac:(CombineCase7 createLastStringPrefixTerm createLastEqualityTerm);
+                set_evars) ltac:(finish honing).
+    Time doOne implement_insert'''
+          ltac:(master_implement_drill
+          ltac:(CombineCase5 StringPrefixIndexUse EqIndexUse)
+          ltac:(CombineCase10 createEarlyStringPrefixTerm createEarlyEqualityTerm)
+          ltac:(CombineCase7 createLastStringPrefixTerm createLastEqualityTerm);
+                set_evars) ltac:(finish honing).
+    Time doOne implement_insert'''
+          ltac:(master_implement_drill
+          ltac:(CombineCase5 StringPrefixIndexUse EqIndexUse)
+          ltac:(CombineCase10 createEarlyStringPrefixTerm createEarlyEqualityTerm)
+          ltac:(CombineCase7 createLastStringPrefixTerm createLastEqualityTerm);
+                set_evars) ltac:(finish honing).
+    apply refine_foldComp; intros ? ?; set_refine_evar.
+    repeat doOne implement_insert'''
+          ltac:(master_implement_drill
+          ltac:(CombineCase5 StringPrefixIndexUse EqIndexUse)
+          ltac:(CombineCase10 createEarlyStringPrefixTerm createEarlyEqualityTerm)
+          ltac:(CombineCase7 createLastStringPrefixTerm createLastEqualityTerm);
+                set_evars) ltac:(finish honing).
+    repeat doOne implement_insert'''
+          ltac:(master_implement_drill
+          ltac:(CombineCase5 StringPrefixIndexUse EqIndexUse)
+          ltac:(CombineCase10 createEarlyStringPrefixTerm createEarlyEqualityTerm)
+          ltac:(CombineCase7 createLastStringPrefixTerm createLastEqualityTerm);
+                set_evars) ltac:(finish honing).
+    repeat doOne implement_insert'''
+          ltac:(master_implement_drill
+          ltac:(CombineCase5 StringPrefixIndexUse EqIndexUse)
+          ltac:(CombineCase10 createEarlyStringPrefixTerm createEarlyEqualityTerm)
+          ltac:(CombineCase7 createLastStringPrefixTerm createLastEqualityTerm);
+                set_evars) ltac:(finish honing).
+    repeat doOne implement_insert'''
+          ltac:(master_implement_drill
+          ltac:(CombineCase5 StringPrefixIndexUse EqIndexUse)
+          ltac:(CombineCase10 createEarlyStringPrefixTerm createEarlyEqualityTerm)
+          ltac:(CombineCase7 createLastStringPrefixTerm createLastEqualityTerm);
+                set_evars) ltac:(finish honing).
+  }
 
   simpl.
-  (* All constraints dropped. *)
-    progress doOne srewrite_each_all drills_each_all finish_each_all.
-    doOne srewrite_each_all drills_each_all finish_each_all.
-    doOne srewrite_each_all drills_each_all finish_each_all.
-    doOne srewrite_each_all drills_each_all finish_each_all.
-    doOne srewrite_each_all drills_each_all finish_each_all.
-    doOne srewrite_each_all drills_each_all finish_each_all.
-    doOne srewrite_each_all drills_each_all finish_each_all.
-    doOne srewrite_each_all drills_each_all finish_each_all.
-    doOne srewrite_each_all drills_each_all finish_each_all.
-    doOne srewrite_each_all drills_each_all finish_each_all.
-    doOne srewrite_each_all drills_each_all finish_each_all.
-    doOne srewrite_each_all drills_each_all finish_each_all.
-    doOne srewrite_each_all drills_each_all finish_each_all.
-    doOne srewrite_each_all drills_each_all finish_each_all.
-    doOne srewrite_each_all drills_each_all finish_each_all.
-    doOne srewrite_each_all drills_each_all finish_each_all.
-    doOne srewrite_each_all drills_each_all finish_each_all.
-    doOne srewrite_each_all drills_each_all finish_each_all.
-    doOne srewrite_each_all drills_each_all finish_each_all.
-    doOne srewrite_each_all drills_each_all finish_each_all.
-    doOne srewrite_each_all drills_each_all finish_each_all.
-    doOne srewrite_each_all drills_each_all finish_each_all.
-    doOne srewrite_each_all drills_each_all finish_each_all.
-    doOne srewrite_each_all drills_each_all finish_each_all.
-    doOne srewrite_each_all drills_each_all finish_each_all.
-    doOne srewrite_each_all drills_each_all finish_each_all.
-  }
-  drop_constraintsfrom_DNS.
-  - doAny drop_constraints
-           master_rewrite_drill ltac:(repeat subst_refine_evar; try finish honing).
-  - doOne drop_constraints
-          master_rewrite_drill ltac:(repeat subst_refine_evar; try finish honing).
-    doOne drop_constraints
-          master_rewrite_drill ltac:(repeat subst_refine_evar; try finish honing).
-    doOne drop_constraints
-          master_rewrite_drill ltac:(repeat subst_refine_evar; try finish honing).
-    doOne drop_constraints
-          master_rewrite_drill ltac:(repeat subst_refine_evar; try finish honing).
-doOne drop_constraints
-          master_rewrite_drill ltac:(repeat subst_refine_evar; try finish honing).
-    doOne drop_constraints
-          master_rewrite_drill ltac:(repeat subst_refine_evar; try finish honing).
-    doOne drop_constraints
-          master_rewrite_drill ltac:(repeat subst_refine_evar; try finish honing).
-    doOne drop_constraints
-          master_rewrite_drill ltac:(repeat subst_refine_evar; try finish honing).
-    doOne drop_constraints
-          master_rewrite_drill ltac:(repeat subst_refine_evar; try finish honing).
-    doOne drop_constraints
-          master_rewrite_drill ltac:(repeat subst_refine_evar; try finish honing).
-    doOne drop_constraints
-          master_rewrite_drill ltac:(repeat subst_refine_evar; try finish honing).
-    doOne drop_constraints
-          master_rewrite_drill ltac:(repeat subst_refine_evar; try finish honing).
-    doOne drop_constraints
-          master_rewrite_drill ltac:(repeat subst_refine_evar; try finish honing).
-    doOne drop_constraints
-          master_rewrite_drill ltac:(repeat subst_refine_evar; try finish honing).
-    doOne drop_constraints
-          master_rewrite_drill ltac:(repeat subst_refine_evar; try finish honing).
-    doOne drop_constraints
-          master_rewrite_drill ltac:(repeat subst_refine_evar; try finish honing).
-    doOne drop_constraints
-          master_rewrite_drill ltac:(repeat subst_refine_evar; try finish honing).
-    doOne drop_constraints
-          master_rewrite_drill ltac:(repeat subst_refine_evar; try finish honing).
-    doOne drop_constraints
-          master_rewrite_drill ltac:(repeat subst_refine_evar; try finish honing).
-    doOne drop_constraints
-          master_rewrite_drill ltac:(repeat subst_refine_evar; try finish honing).
-    doOne drop_constraints
-          master_rewrite_drill ltac:(repeat subst_refine_evar; try finish honing).
-    doOne drop_constraints
-          master_rewrite_drill ltac:(repeat subst_refine_evar; try finish honing).
-    doOne drop_constraints
-          master_rewrite_drill ltac:(repeat subst_refine_evar; try finish honing).
-    doOne drop_constraints
-          master_rewrite_drill ltac:(repeat subst_refine_evar; try finish honing).
-    doOne drop_constraints
-          master_rewrite_drill ltac:(repeat subst_refine_evar; try finish honing).
-    doOne drop_constraints
-          master_rewrite_drill ltac:(repeat subst_refine_evar; try finish honing).
-    doOne drop_constraints
-          master_rewrite_drill ltac:(repeat subst_refine_evar; try finish honing).
-    doOne drop_constraints
-          master_rewrite_drill ltac:(repeat subst_refine_evar; try finish honing).
-    doOne drop_constraints
-          master_rewrite_drill ltac:(repeat subst_refine_evar; try finish honing).
-    doOne drop_constraints
-          master_rewrite_drill ltac:(repeat subst_refine_evar; try finish honing).
-    doOne drop_constraints
-          master_rewrite_drill ltac:(repeat subst_refine_evar; try finish honing).
-    doOne drop_constraints
-          master_rewrite_drill ltac:(repeat subst_refine_evar; try finish honing).
-    doOne drop_constraints
-          master_rewrite_drill ltac:(repeat subst_refine_evar; try finish honing).
-    doOne drop_constraints
-          master_rewrite_drill ltac:(repeat subst_refine_evar; try finish honing).
-    doOne drop_constraints
-          master_rewrite_drill ltac:(repeat subst_refine_evar; try finish honing).
-        doOne drop_constraints
-          master_rewrite_drill ltac:(repeat subst_refine_evar; try finish honing).
-  - hone method "AddData".
-    simplify with monad laws; etransitivity; set_evars.
-    doAny simplify_queries
-          Finite_AbsR_rewrite_drill ltac:(repeat subst_refine_evar; try finish honing).
-    doOne srewrite_each_all drills_each_all finish_each_all.
-    doOne srewrite_each_all drills_each_all finish_each_all.
-    doOne srewrite_each_all drills_each_all finish_each_all.
-    doOne srewrite_each_all drills_each_all finish_each_all.
-    setoid_rewrite refine_count_constraint_broken.
-    repeat doOne srewrite_each_all drills_each_all finish_each_all.
-    repeat doOne srewrite_each_all drills_each_all finish_each_all.
-    make_simple_indexes ({|prim_fst := [("FindPrefixIndex", Fin.F1)];
-                           prim_snd := () |} : prim_prod (list (string * Fin.t 6)) ())
-                        ltac:(CombineCase6 BuildEarlyFindPrefixIndex ltac:(LastCombineCase6 BuildEarlyEqualityIndex))
-                               ltac:(CombineCase5 BuildLastFindPrefixIndex ltac:(LastCombineCase5 BuildLastEqualityIndex)).
-    + plan EqIndexUse createEarlyEqualityTerm createLastEqualityTerm
-           EqIndexUse_dep createEarlyEqualityTerm_dep createLastEqualityTerm_dep.
-    + repeat doOne implement_insert''
-            ltac:(master_implement_drill EqIndexUse createEarlyEqualityTerm createLastEqualityTerm; set_evars) ltac:(finish honing).
-    + doOne implement_insert''
-            ltac:(master_implement_drill EqIndexUse createEarlyEqualityTerm createLastEqualityTerm; set_evars) ltac:(finish honing).
-      doOne implement_insert''
-            ltac:(master_implement_drill EqIndexUse createEarlyEqualityTerm createLastEqualityTerm; set_evars) ltac:(finish honing).
-      doOne implement_insert''
-            ltac:(master_implement_drill EqIndexUse createEarlyEqualityTerm createLastEqualityTerm; set_evars) ltac:(finish honing).
-      doOne implement_insert''
-            ltac:(master_implement_drill EqIndexUse createEarlyEqualityTerm createLastEqualityTerm; set_evars) ltac:(finish honing).
-      doOne implement_insert''
-            ltac:(master_implement_drill EqIndexUse createEarlyEqualityTerm createLastEqualityTerm; set_evars) ltac:(finish honing).
-      doOne implement_insert''
-            ltac:(master_implement_drill EqIndexUse createEarlyEqualityTerm createLastEqualityTerm; set_evars) ltac:(finish honing).
-      doOne implement_insert''
-            ltac:(master_implement_drill EqIndexUse createEarlyEqualityTerm createLastEqualityTerm; set_evars) ltac:(finish honing).
-      doOne implement_insert''
-            ltac:(master_implement_drill EqIndexUse createEarlyEqualityTerm createLastEqualityTerm; set_evars) ltac:(finish honing).
-      doOne implement_insert''
-            ltac:(master_implement_drill EqIndexUse createEarlyEqualityTerm createLastEqualityTerm; set_evars) ltac:(finish honing).
-      doOne implement_insert''
-            ltac:(master_implement_drill EqIndexUse createEarlyEqualityTerm createLastEqualityTerm; set_evars) ltac:(finish honing).
-      doOne implement_insert''
-            ltac:(master_implement_drill EqIndexUse createEarlyEqualityTerm createLastEqualityTerm; set_evars) ltac:(finish honing).
-      doOne implement_insert''
-            ltac:(master_implement_drill EqIndexUse createEarlyEqualityTerm createLastEqualityTerm; set_evars) ltac:(finish honing).
-      doOne implement_insert''
-            ltac:(master_implement_drill EqIndexUse createEarlyEqualityTerm createLastEqualityTerm; set_evars) ltac:(finish honing).
-      doOne implement_insert''
-            ltac:(master_implement_drill EqIndexUse createEarlyEqualityTerm createLastEqualityTerm; set_evars) ltac:(finish honing).
-      doOne implement_insert''
-            ltac:(master_implement_drill EqIndexUse createEarlyEqualityTerm createLastEqualityTerm; set_evars) ltac:(finish honing).
-      doOne implement_insert''
-            ltac:(master_implement_drill EqIndexUse createEarlyEqualityTerm createLastEqualityTerm; set_evars) ltac:(finish honing).
-      doOne implement_insert''
-            ltac:(master_implement_drill EqIndexUse createEarlyEqualityTerm createLastEqualityTerm; set_evars) ltac:(finish honing).
-doOne implement_insert''
-            ltac:(master_implement_drill EqIndexUse createEarlyEqualityTerm createLastEqualityTerm; set_evars) ltac:(finish honing).
-      doOne implement_insert''
-            ltac:(master_implement_drill EqIndexUse createEarlyEqualityTerm createLastEqualityTerm; set_evars) ltac:(finish honing).
-
-
-      doOne implement_insert''
-            ltac:(master_implement_drill EqIndexUse createEarlyEqualityTerm createLastEqualityTerm; set_evars) ltac:(finish honing).
-      doOne implement_insert''
-            ltac:(master_implement_drill EqIndexUse createEarlyEqualityTerm createLastEqualityTerm; set_evars) ltac:(finish honing).
-      doOne implement_insert''
-            ltac:(master_implement_drill EqIndexUse createEarlyEqualityTerm createLastEqualityTerm; set_evars) ltac:(finish honing).
-      doOne implement_insert''
-            ltac:(master_implement_drill EqIndexUse createEarlyEqualityTerm createLastEqualityTerm; set_evars) ltac:(finish honing).
-      doOne implement_insert''
-            ltac:(master_implement_drill EqIndexUse createEarlyEqualityTerm createLastEqualityTerm; set_evars) ltac:(finish honing).
-      doOne implement_insert''
-            ltac:(master_implement_drill EqIndexUse createEarlyEqualityTerm createLastEqualityTerm; set_evars) ltac:(finish honing).
-      doOne implement_insert''
-            ltac:(master_implement_drill EqIndexUse createEarlyEqualityTerm createLastEqualityTerm; set_evars) ltac:(finish honing).
-      doOne implement_insert''
-            ltac:(master_implement_drill EqIndexUse createEarlyEqualityTerm createLastEqualityTerm; set_evars) ltac:(finish honing).
-      doOne implement_insert''
-            ltac:(master_implement_drill EqIndexUse createEarlyEqualityTerm createLastEqualityTerm; set_evars) ltac:(finish honing).
-      doOne implement_insert''
-            ltac:(master_implement_drill EqIndexUse createEarlyEqualityTerm createLastEqualityTerm; set_evars) ltac:(finish honing).
-      doOne implement_insert''
-            ltac:(master_implement_drill EqIndexUse createEarlyEqualityTerm createLastEqualityTerm; set_evars) ltac:(finish honing).
-      doOne implement_insert''
-            ltac:(master_implement_drill EqIndexUse createEarlyEqualityTerm createLastEqualityTerm; set_evars) ltac:(finish honing).
-      doOne implement_insert''
-            ltac:(master_implement_drill EqIndexUse createEarlyEqualityTerm createLastEqualityTerm; set_evars) ltac:(finish honing).
-      doOne implement_insert''
-            ltac:(master_implement_drill EqIndexUse createEarlyEqualityTerm createLastEqualityTerm; set_evars) ltac:(finish honing).
-      doOne implement_insert''
-            ltac:(master_implement_drill EqIndexUse createEarlyEqualityTerm createLastEqualityTerm; set_evars) ltac:(finish honing).
-      doOne implement_insert''
-            ltac:(master_implement_drill EqIndexUse createEarlyEqualityTerm createLastEqualityTerm; set_evars) ltac:(finish honing).
-      Focused_refine_TopMost_Query.
-      implement_In_opt.
-      repeat progress distribute_filters_to_joins.
-      implement_filters_with_find
-        ltac:(find_simple_search_term ltac:(CombineCase5 PrefixIndexUse EqIndexUse)
-                      ltac:(CombineCase10 createEarlyPrefixTerm createEarlyEqualityTerm)
-                             ltac:(CombineCase7 createLastPrefixTerm createLastEqualityTerm))
-               ltac:(find_simple_search_term_dep
-                       ltac:(CombineCase7 PrefixIndexUse_dep EqIndexUse_dep)
-                              ltac:(CombineCase11 createEarlyPrefixTerm_dep createEarlyEqualityTerm_dep)
-                                     ltac:(CombineCase8 createLastPrefixTerm_dep createLastEqualityTerm_dep)).
-
-
-
-      doOne implement_insert''
-            ltac:(master_implement_drill EqIndexUse createEarlyEqualityTerm createLastEqualityTerm; set_evars) ltac:(finish honing).
-      implement_In_opt.
-      repeat progress distribute_filters_to_joins.
-      setoid_rewrite
-      match goal with
-  | [H : @DelegateToBag_AbsR ?qs_schema ?indexes ?r_o ?r_n
-     |- refine (UnConstrQuery_In (ResultT := ?resultT) ?r_o ?idx ?f) _ ] =>
-    etransitivity;
-      [ let H' := eval simpl in (refine_Filtered_Query_In_Enumerate H (idx := idx) f) in
-            apply H'
-      | apply refine_under_bind; intros; implement_In_opt' ]
-
-  | [H : @DelegateToBag_AbsR ?qs_schema ?indexes ?r_o ?r_n
-     |- refine (List_Query_In ?b (fun b : ?QueryT => Where (@?P b) (@?resultComp b))) _ ] =>
-    etransitivity;
-      [ let H' := eval simpl in (@refine_List_Query_In_Where QueryT _ b P resultComp _) in
-            apply H'
-      | implement_In_opt'; implement_In_opt' ] end.
-
-
-    +  unfold SearchUpdateTerm in Index; simpl in Index.
-       simpl.
-Finish_Master ltac:(CombineCase6 BuildEarlyTrieBag  BuildEarlyBag )
-                           ltac:(CombineCase5 BuildLastTrieBag BuildLastBag).
-Time Defined. *)
-
-End BinaryDns.
-
-(*
-Definition DnsSig : ADTSig :=
-  ADTsignature {
-      Constructor "Init" : rep,
-      Method "AddData" : rep * resourceRecord -> rep * bool,
-      Method "Process" : rep * packet -> rep * packet
-    }.
-
-
-Definition DnsSpec (recurseDepth : nat) : ADT DnsSig :=
-  Def ADT {
-    rep := QueryStructure DnsSchema,
-
-    Def Constructor "Init" : rep := empty,,
-
-    (* in start honing querystructure, it inserts constraints before *)
-    (* every insert / decision procedure *)
-
-    Def Method1 "AddData" (this : rep) (t : resourceRecord) : rep * bool :=
-      Insert t into this!sRRecords,
-
-    Def Method1 "Process" (this : rep) (p : packet) : rep * packet :=
-        Repeat recurseDepth initializing n with p!"question"!"qname"
-               defaulting rec with (ret (buildempty true ``"ServFail" p)) (* Bottoming out w/o an answer signifies a server failure error. *)
-        {{ results <- MaxElements (fun r r' : resourceRecord => IsPrefix r!sNAME r'!sNAME)
-                             (For (r in this!sRRecords)      (* Bind a list of all the DNS entries *)
-                               Where (IsPrefix r!sNAME n)   (* prefixed with [n] to [rs] *)
-                               Return r);
-            If (is_empty results) (* Are there any matching records? *)
-            Then ret (buildempty true ``"NXDomain" p) (* No matching records, set name error *)
-            Else
-            (IfDec (Forall (fun r : resourceRecord => n = r!sNAME) results) (* If the record's QNAME is an exact match  *)
-              Then
-              b <- SingletonSet (fun b : CNAME_Record =>      (* If the record is a CNAME, *)
-                                   List.In (A := resourceRecord) b results
-                                   /\ p!"question"!"qtype" <> QType_inj CNAME); (* and a non-CNAME was requested*)
-                Ifopt b as b'
-                Then  (* only one matching CNAME record *)
-                  p' <- rec b'!sRDATA; (* Recursively find records matching the CNAME *)
-                  ret (add_answer p' b') (* Add the CNAME RR to the answer section *)
-                Else     (* Copy the records with the correct QTYPE into the answer *)
-                         (* section of an empty response *)
-                (results <- ⟦ element in results | QType_match (element!sTYPE) (p!"question"!"qtype") ⟧;
-                  ret (add_answers results (buildempty true ``"NoError" p)))
-              Else (* prefix but record's QNAME not an exact match *)
-                (* return all the prefix records that are nameserver records -- *)
-                (* ask the authoritative servers *)
-              (ns_results <- { ns_results | forall x : NS_Record, List.In x ns_results <-> List.In (A := resourceRecord) x results };
-                 (* Append all the glue records to the additional section. *)
-                 glue_results <- For (rRec in this!sRRecords)
-                                 Where (List.In rRec!sNAME (map (fun r : NS_Record => r!sRDATA) ns_results))
-                                 Return rRec;
-                 ret (add_additionals glue_results (add_nses (map VariantResourceRecord2RRecord ns_results) (buildempty true ``"NoError" p)))))
-          }} >>= fun p => ret (this, p)}. *)
-
-Local Arguments packet : simpl never.
-
-(* Making fold_list Opaque greatly speeds up setoid_rewriting. *)
-Opaque fold_left.
-
-(* Need to update derivation to work with arbitrary recursion depth. *)
-
-(*Theorem DnsManual (recurseDepth : nat) :
-  FullySharpened (DnsSpec recurseDepth).
-Proof.
-  start sharpening ADT; unfold DnsSpec.
-  simpl; pose_string_hyps; pose_heading_hyps.
-  hone method "Process".
-  simpl in *.
-  { simplify with monad laws.
-
-    doOne srewrite_each_all drills_each_all finish_each_all.
-    doOne srewrite_each_all drills_each_all finish_each_all.
-    doOne srewrite_each_all drills_each_all finish_each_all.
-    doOne srewrite_each_all drills_each_all finish_each_all.
-    doOne srewrite_each_all drills_each_all finish_each_all.
-    doOne srewrite_each_all drills_each_all finish_each_all.
-    doOne srewrite_each_all drills_each_all finish_each_all.
-    doOne srewrite_each_all drills_each_all finish_each_all.
-    doOne srewrite_each_all drills_each_all finish_each_all.
-    doOne srewrite_each_all drills_each_all finish_each_all.
-    doOne srewrite_each_all drills_each_all finish_each_all.
-    doOne srewrite_each_all drills_each_all finish_each_all.
-    doOne srewrite_each_all drills_each_all finish_each_all.
-    doOne srewrite_each_all drills_each_all finish_each_all.
-    doOne srewrite_each_all drills_each_all finish_each_all.
-    doOne srewrite_each_all drills_each_all finish_each_all.
-    doOne srewrite_each_all drills_each_all finish_each_all.
-    doOne srewrite_each_all drills_each_all finish_each_all.
-    doOne srewrite_each_all drills_each_all finish_each_all.
-    doOne srewrite_each_all drills_each_all finish_each_all.
-    doOne srewrite_each_all drills_each_all finish_each_all.
-    doOne srewrite_each_all drills_each_all finish_each_all.
-    doOne srewrite_each_all drills_each_all finish_each_all.
-    doOne srewrite_each_all drills_each_all finish_each_all.
-    doOne srewrite_each_all drills_each_all finish_each_all.
-    doOne srewrite_each_all drills_each_all finish_each_all.
-    doOne srewrite_each_all drills_each_all finish_each_all.
-    doOne srewrite_each_all drills_each_all finish_each_all.
-    doOne srewrite_each_all drills_each_all finish_each_all.
-    doOne srewrite_each_all drills_each_all finish_each_all.
-    doOne srewrite_each_all drills_each_all finish_each_all.
-    doOne srewrite_each_all drills_each_all finish_each_all.
-    doOne srewrite_each_all drills_each_all finish_each_all.
-    doOne srewrite_each_all drills_each_all finish_each_all.
-    doOne srewrite_each_all drills_each_all finish_each_all.
-    doOne srewrite_each_all drills_each_all finish_each_all.
-  }
-  drop_constraintsfrom_DNS.
-  - doAny drop_constraints
-           master_rewrite_drill ltac:(repeat subst_refine_evar; try finish honing).
-  - doOne drop_constraints
-          master_rewrite_drill ltac:(repeat subst_refine_evar; try finish honing).
-    doOne drop_constraints
-          master_rewrite_drill ltac:(repeat subst_refine_evar; try finish honing).
-    doOne drop_constraints
-          master_rewrite_drill ltac:(repeat subst_refine_evar; try finish honing).
-    doOne drop_constraints
-          master_rewrite_drill ltac:(repeat subst_refine_evar; try finish honing).
-doOne drop_constraints
-          master_rewrite_drill ltac:(repeat subst_refine_evar; try finish honing).
-    doOne drop_constraints
-          master_rewrite_drill ltac:(repeat subst_refine_evar; try finish honing).
-    doOne drop_constraints
-          master_rewrite_drill ltac:(repeat subst_refine_evar; try finish honing).
-    doOne drop_constraints
-          master_rewrite_drill ltac:(repeat subst_refine_evar; try finish honing).
-    doOne drop_constraints
-          master_rewrite_drill ltac:(repeat subst_refine_evar; try finish honing).
-    doOne drop_constraints
-          master_rewrite_drill ltac:(repeat subst_refine_evar; try finish honing).
-    doOne drop_constraints
-          master_rewrite_drill ltac:(repeat subst_refine_evar; try finish honing).
-    doOne drop_constraints
-          master_rewrite_drill ltac:(repeat subst_refine_evar; try finish honing).
-    doOne drop_constraints
-          master_rewrite_drill ltac:(repeat subst_refine_evar; try finish honing).
-    doOne drop_constraints
-          master_rewrite_drill ltac:(repeat subst_refine_evar; try finish honing).
-    doOne drop_constraints
-          master_rewrite_drill ltac:(repeat subst_refine_evar; try finish honing).
-    doOne drop_constraints
-          master_rewrite_drill ltac:(repeat subst_refine_evar; try finish honing).
-    doOne drop_constraints
-          master_rewrite_drill ltac:(repeat subst_refine_evar; try finish honing).
-    doOne drop_constraints
-          master_rewrite_drill ltac:(repeat subst_refine_evar; try finish honing).
-    doOne drop_constraints
-          master_rewrite_drill ltac:(repeat subst_refine_evar; try finish honing).
-    doOne drop_constraints
-          master_rewrite_drill ltac:(repeat subst_refine_evar; try finish honing).
-    doOne drop_constraints
-          master_rewrite_drill ltac:(repeat subst_refine_evar; try finish honing).
-    doOne drop_constraints
-          master_rewrite_drill ltac:(repeat subst_refine_evar; try finish honing).
-    doOne drop_constraints
-          master_rewrite_drill ltac:(repeat subst_refine_evar; try finish honing).
-    doOne drop_constraints
-          master_rewrite_drill ltac:(repeat subst_refine_evar; try finish honing).
-    doOne drop_constraints
-          master_rewrite_drill ltac:(repeat subst_refine_evar; try finish honing).
-    doOne drop_constraints
-          master_rewrite_drill ltac:(repeat subst_refine_evar; try finish honing).
-    doOne drop_constraints
-          master_rewrite_drill ltac:(repeat subst_refine_evar; try finish honing).
-    doOne drop_constraints
-          master_rewrite_drill ltac:(repeat subst_refine_evar; try finish honing).
-    doOne drop_constraints
-          master_rewrite_drill ltac:(repeat subst_refine_evar; try finish honing).
-    doOne drop_constraints
-          master_rewrite_drill ltac:(repeat subst_refine_evar; try finish honing).
-    doOne drop_constraints
-          master_rewrite_drill ltac:(repeat subst_refine_evar; try finish honing).
-    doOne drop_constraints
-          master_rewrite_drill ltac:(repeat subst_refine_evar; try finish honing).
-    doOne drop_constraints
-          master_rewrite_drill ltac:(repeat subst_refine_evar; try finish honing).
-    doOne drop_constraints
-          master_rewrite_drill ltac:(repeat subst_refine_evar; try finish honing).
-    doOne drop_constraints
-          master_rewrite_drill ltac:(repeat subst_refine_evar; try finish honing).
-        doOne drop_constraints
-          master_rewrite_drill ltac:(repeat subst_refine_evar; try finish honing).
-  - hone method "AddData".
-    simplify with monad laws; etransitivity; set_evars.
-    doAny simplify_queries
-          Finite_AbsR_rewrite_drill ltac:(repeat subst_refine_evar; try finish honing).
-    doOne srewrite_each_all drills_each_all finish_each_all.
-    doOne srewrite_each_all drills_each_all finish_each_all.
-    doOne srewrite_each_all drills_each_all finish_each_all.
-    doOne srewrite_each_all drills_each_all finish_each_all.
-    setoid_rewrite refine_count_constraint_broken.
-    repeat doOne srewrite_each_all drills_each_all finish_each_all.
-    repeat doOne srewrite_each_all drills_each_all finish_each_all.
-    make_simple_indexes ({|prim_fst := [("FindPrefixIndex", Fin.F1)];
-                           prim_snd := () |} : prim_prod (list (string * Fin.t 6)) ())
-                        ltac:(CombineCase6 BuildEarlyFindPrefixIndex ltac:(LastCombineCase6 BuildEarlyEqualityIndex))
-                               ltac:(CombineCase5 BuildLastFindPrefixIndex ltac:(LastCombineCase5 BuildLastEqualityIndex)).
-    + plan EqIndexUse createEarlyEqualityTerm createLastEqualityTerm
-           EqIndexUse_dep createEarlyEqualityTerm_dep createLastEqualityTerm_dep.
-    + repeat doOne implement_insert''
-            ltac:(master_implement_drill EqIndexUse createEarlyEqualityTerm createLastEqualityTerm; set_evars) ltac:(finish honing).
-    + doOne implement_insert''
-            ltac:(master_implement_drill EqIndexUse createEarlyEqualityTerm createLastEqualityTerm; set_evars) ltac:(finish honing).
-      doOne implement_insert''
-            ltac:(master_implement_drill EqIndexUse createEarlyEqualityTerm createLastEqualityTerm; set_evars) ltac:(finish honing).
-      doOne implement_insert''
-            ltac:(master_implement_drill EqIndexUse createEarlyEqualityTerm createLastEqualityTerm; set_evars) ltac:(finish honing).
-      doOne implement_insert''
-            ltac:(master_implement_drill EqIndexUse createEarlyEqualityTerm createLastEqualityTerm; set_evars) ltac:(finish honing).
-      doOne implement_insert''
-            ltac:(master_implement_drill EqIndexUse createEarlyEqualityTerm createLastEqualityTerm; set_evars) ltac:(finish honing).
-      doOne implement_insert''
-            ltac:(master_implement_drill EqIndexUse createEarlyEqualityTerm createLastEqualityTerm; set_evars) ltac:(finish honing).
-      doOne implement_insert''
-            ltac:(master_implement_drill EqIndexUse createEarlyEqualityTerm createLastEqualityTerm; set_evars) ltac:(finish honing).
-      doOne implement_insert''
-            ltac:(master_implement_drill EqIndexUse createEarlyEqualityTerm createLastEqualityTerm; set_evars) ltac:(finish honing).
-      doOne implement_insert''
-            ltac:(master_implement_drill EqIndexUse createEarlyEqualityTerm createLastEqualityTerm; set_evars) ltac:(finish honing).
-      doOne implement_insert''
-            ltac:(master_implement_drill EqIndexUse createEarlyEqualityTerm createLastEqualityTerm; set_evars) ltac:(finish honing).
-      doOne implement_insert''
-            ltac:(master_implement_drill EqIndexUse createEarlyEqualityTerm createLastEqualityTerm; set_evars) ltac:(finish honing).
-      doOne implement_insert''
-            ltac:(master_implement_drill EqIndexUse createEarlyEqualityTerm createLastEqualityTerm; set_evars) ltac:(finish honing).
-      doOne implement_insert''
-            ltac:(master_implement_drill EqIndexUse createEarlyEqualityTerm createLastEqualityTerm; set_evars) ltac:(finish honing).
-      doOne implement_insert''
-            ltac:(master_implement_drill EqIndexUse createEarlyEqualityTerm createLastEqualityTerm; set_evars) ltac:(finish honing).
-      doOne implement_insert''
-            ltac:(master_implement_drill EqIndexUse createEarlyEqualityTerm createLastEqualityTerm; set_evars) ltac:(finish honing).
-      doOne implement_insert''
-            ltac:(master_implement_drill EqIndexUse createEarlyEqualityTerm createLastEqualityTerm; set_evars) ltac:(finish honing).
-      doOne implement_insert''
-            ltac:(master_implement_drill EqIndexUse createEarlyEqualityTerm createLastEqualityTerm; set_evars) ltac:(finish honing).
-doOne implement_insert''
-            ltac:(master_implement_drill EqIndexUse createEarlyEqualityTerm createLastEqualityTerm; set_evars) ltac:(finish honing).
-      doOne implement_insert''
-            ltac:(master_implement_drill EqIndexUse createEarlyEqualityTerm createLastEqualityTerm; set_evars) ltac:(finish honing).
-
-
-      doOne implement_insert''
-            ltac:(master_implement_drill EqIndexUse createEarlyEqualityTerm createLastEqualityTerm; set_evars) ltac:(finish honing).
-      doOne implement_insert''
-            ltac:(master_implement_drill EqIndexUse createEarlyEqualityTerm createLastEqualityTerm; set_evars) ltac:(finish honing).
-      doOne implement_insert''
-            ltac:(master_implement_drill EqIndexUse createEarlyEqualityTerm createLastEqualityTerm; set_evars) ltac:(finish honing).
-      doOne implement_insert''
-            ltac:(master_implement_drill EqIndexUse createEarlyEqualityTerm createLastEqualityTerm; set_evars) ltac:(finish honing).
-      doOne implement_insert''
-            ltac:(master_implement_drill EqIndexUse createEarlyEqualityTerm createLastEqualityTerm; set_evars) ltac:(finish honing).
-      doOne implement_insert''
-            ltac:(master_implement_drill EqIndexUse createEarlyEqualityTerm createLastEqualityTerm; set_evars) ltac:(finish honing).
-      doOne implement_insert''
-            ltac:(master_implement_drill EqIndexUse createEarlyEqualityTerm createLastEqualityTerm; set_evars) ltac:(finish honing).
-      doOne implement_insert''
-            ltac:(master_implement_drill EqIndexUse createEarlyEqualityTerm createLastEqualityTerm; set_evars) ltac:(finish honing).
-      doOne implement_insert''
-            ltac:(master_implement_drill EqIndexUse createEarlyEqualityTerm createLastEqualityTerm; set_evars) ltac:(finish honing).
-      doOne implement_insert''
-            ltac:(master_implement_drill EqIndexUse createEarlyEqualityTerm createLastEqualityTerm; set_evars) ltac:(finish honing).
-      doOne implement_insert''
-            ltac:(master_implement_drill EqIndexUse createEarlyEqualityTerm createLastEqualityTerm; set_evars) ltac:(finish honing).
-      doOne implement_insert''
-            ltac:(master_implement_drill EqIndexUse createEarlyEqualityTerm createLastEqualityTerm; set_evars) ltac:(finish honing).
-      doOne implement_insert''
-            ltac:(master_implement_drill EqIndexUse createEarlyEqualityTerm createLastEqualityTerm; set_evars) ltac:(finish honing).
-      doOne implement_insert''
-            ltac:(master_implement_drill EqIndexUse createEarlyEqualityTerm createLastEqualityTerm; set_evars) ltac:(finish honing).
-      doOne implement_insert''
-            ltac:(master_implement_drill EqIndexUse createEarlyEqualityTerm createLastEqualityTerm; set_evars) ltac:(finish honing).
-      doOne implement_insert''
-            ltac:(master_implement_drill EqIndexUse createEarlyEqualityTerm createLastEqualityTerm; set_evars) ltac:(finish honing).
-      Focused_refine_TopMost_Query.
-      implement_In_opt.
-      repeat progress distribute_filters_to_joins.
-      implement_filters_with_find
-        ltac:(find_simple_search_term ltac:(CombineCase5 PrefixIndexUse EqIndexUse)
-                      ltac:(CombineCase10 createEarlyPrefixTerm createEarlyEqualityTerm)
-                             ltac:(CombineCase7 createLastPrefixTerm createLastEqualityTerm))
-               ltac:(find_simple_search_term_dep
-                       ltac:(CombineCase7 PrefixIndexUse_dep EqIndexUse_dep)
-                              ltac:(CombineCase11 createEarlyPrefixTerm_dep createEarlyEqualityTerm_dep)
-                                     ltac:(CombineCase8 createLastPrefixTerm_dep createLastEqualityTerm_dep)).
-
-
-
-      doOne implement_insert''
-            ltac:(master_implement_drill EqIndexUse createEarlyEqualityTerm createLastEqualityTerm; set_evars) ltac:(finish honing).
-      implement_In_opt.
-      repeat progress distribute_filters_to_joins.
-      setoid_rewrite
-      match goal with
-  | [H : @DelegateToBag_AbsR ?qs_schema ?indexes ?r_o ?r_n
-     |- refine (UnConstrQuery_In (ResultT := ?resultT) ?r_o ?idx ?f) _ ] =>
-    etransitivity;
-      [ let H' := eval simpl in (refine_Filtered_Query_In_Enumerate H (idx := idx) f) in
-            apply H'
-      | apply refine_under_bind; intros; implement_In_opt' ]
-
-  | [H : @DelegateToBag_AbsR ?qs_schema ?indexes ?r_o ?r_n
-     |- refine (List_Query_In ?b (fun b : ?QueryT => Where (@?P b) (@?resultComp b))) _ ] =>
-    etransitivity;
-      [ let H' := eval simpl in (@refine_List_Query_In_Where QueryT _ b P resultComp _) in
-            apply H'
-      | implement_In_opt'; implement_In_opt' ] end.
-
-
-    +  unfold SearchUpdateTerm in Index; simpl in Index.
-       simpl.
-Finish_Master ltac:(CombineCase6 BuildEarlyTrieBag  BuildEarlyBag )
-                           ltac:(CombineCase5 BuildLastTrieBag BuildLastBag).
-Time Defined.
+  apply reflexivityT.
+  Time Defined.
 
 Time Definition DNSImpl := Eval simpl in (projT1 DnsManual).
+Print DNSImpl.
 
-Print DNSImpl. *)
-
-(* TODO extraction, examples/messagesextraction.v *)
+End BinaryDns.
