src/BinEncoders/Env/Examples/SimpleDnsOpt.v
@@ -1,4 +1,4 @@
-Require Import
+vRequire Import
         Coq.Strings.String
         Coq.Arith.Mult
         Coq.Vectors.Vector.
